enforcing capitalization of identifiers even for types ... no longer any distinction among the strata; --universes

src/ocaml-output/FStar_Parser_Env.ml
@@ -2,7 +2,7 @@
 open Prims
 # 34 "FStar.Parser.Env.fst"
 type env =
-{curmodule : FStar_Ident.lident Prims.option; modules : (FStar_Ident.lident * FStar_Syntax_Syntax.modul) Prims.list; open_namespaces : FStar_Ident.lident Prims.list; sigaccum : FStar_Syntax_Syntax.sigelts; localbindings : (FStar_Ident.ident * FStar_Syntax_Syntax.bv) Prims.list; recbindings : (FStar_Ident.ident * FStar_Ident.lident) Prims.list; sigmap : (FStar_Syntax_Syntax.sigelt * Prims.bool) FStar_Util.smap Prims.list; default_result_effect : FStar_Ident.lident; iface : Prims.bool; admitted_iface : Prims.bool; expect_typ : Prims.bool}
+{curmodule : FStar_Ident.lident Prims.option; modules : (FStar_Ident.lident * FStar_Syntax_Syntax.modul) Prims.list; open_namespaces : FStar_Ident.lident Prims.list; sigaccum : FStar_Syntax_Syntax.sigelts; localbindings : (FStar_Ident.ident * FStar_Syntax_Syntax.bv) Prims.list; recbindings : (FStar_Ident.ident * FStar_Ident.lid * FStar_Syntax_Syntax.delta_depth) Prims.list; sigmap : (FStar_Syntax_Syntax.sigelt * Prims.bool) FStar_Util.smap Prims.list; default_result_effect : FStar_Ident.lident; iface : Prims.bool; admitted_iface : Prims.bool; expect_typ : Prims.bool}
 
 # 34 "FStar.Parser.Env.fst"
 let is_Mkenv : env  ->  Prims.bool = (Obj.magic ((fun _ -> (FStar_All.failwith "Not yet implemented:is_Mkenv"))))
@@ -282,11 +282,11 @@ end
 (
 # 205 "FStar.Parser.Env.fst"
 let recname = (qualify env lid.FStar_Ident.ident)
-in (FStar_Util.find_map env.recbindings (fun _50_209 -> (match (_50_209) with
-| (id, l) -> begin
+in (FStar_Util.find_map env.recbindings (fun _50_210 -> (match (_50_210) with
+| (id, l, dd) -> begin
 if (id.FStar_Ident.idText = lid.FStar_Ident.ident.FStar_Ident.idText) then begin
 (let _131_176 = (let _131_175 = (let _131_174 = (FStar_Ident.set_lid_range l (FStar_Ident.range_of_lid lid))
-in (FStar_Syntax_Syntax.fvar _131_174 FStar_Syntax_Syntax.Delta_equational None))
+in (FStar_Syntax_Syntax.fvar _131_174 dd None))
 in Term_name (_131_175))
 in Some (_131_176))
 end else begin
@@ -295,14 +295,14 @@ end
 end))))
 end)
 end
-| _50_211 -> begin
+| _50_212 -> begin
 None
 end)
 in (match (found_id) with
-| Some (_50_214) -> begin
+| Some (_50_215) -> begin
 found_id
 end
-| _50_217 -> begin
+| _50_218 -> begin
 (resolve_in_open_namespaces env lid find_in_sig)
 end))))
 
@@ -311,7 +311,7 @@ let try_lookup_effect_name' : Prims.bool  ->  env  ->  FStar_Ident.lident  ->  (
 | Some (Eff_name (o, l)) -> begin
 Some ((o, l))
 end
-| _50_227 -> begin
+| _50_228 -> begin
 None
 end))
 
@@ -320,16 +320,16 @@ let try_lookup_effect_name : env  ->  FStar_Ident.lident  ->  FStar_Ident.lident
 | Some (o, l) -> begin
 Some (l)
 end
-| _50_235 -> begin
+| _50_236 -> begin
 None
 end))
 
 # 224 "FStar.Parser.Env.fst"
 let try_lookup_effect_defn : env  ->  FStar_Ident.lident  ->  FStar_Syntax_Syntax.eff_decl Prims.option = (fun env l -> (match ((try_lookup_effect_name' (not (env.iface)) env l)) with
-| Some (FStar_Syntax_Syntax.Sig_new_effect (ne, _50_240), _50_244) -> begin
+| Some (FStar_Syntax_Syntax.Sig_new_effect (ne, _50_241), _50_245) -> begin
 Some (ne)
 end
-| _50_248 -> begin
+| _50_249 -> begin
 None
 end))
 
@@ -338,7 +338,7 @@ let is_effect_name : env  ->  FStar_Ident.lident  ->  Prims.bool = (fun env lid 
 | None -> begin
 false
 end
-| Some (_50_253) -> begin
+| Some (_50_254) -> begin
 true
 end))
 
@@ -347,26 +347,26 @@ let lookup_letbinding_quals : env  ->  FStar_Ident.lident  ->  FStar_Syntax_Synt
 # 234 "FStar.Parser.Env.fst"
 let find_in_sig = (fun lid -> (match ((let _131_201 = (sigmap env)
 in (FStar_Util.smap_try_find _131_201 lid.FStar_Ident.str))) with
-| Some (FStar_Syntax_Syntax.Sig_declare_typ (lid, _50_261, _50_263, quals, _50_266), _50_270) -> begin
+| Some (FStar_Syntax_Syntax.Sig_declare_typ (lid, _50_262, _50_264, quals, _50_267), _50_271) -> begin
 Some (quals)
 end
-| _50_274 -> begin
+| _50_275 -> begin
 None
 end))
 in (match ((resolve_in_open_namespaces env lid find_in_sig)) with
 | Some (quals) -> begin
 quals
 end
-| _50_278 -> begin
+| _50_279 -> begin
 []
 end)))
 
 # 242 "FStar.Parser.Env.fst"
-let try_lookup_module : env  ->  Prims.string Prims.list  ->  FStar_Syntax_Syntax.modul Prims.option = (fun env path -> (match ((FStar_List.tryFind (fun _50_283 -> (match (_50_283) with
+let try_lookup_module : env  ->  Prims.string Prims.list  ->  FStar_Syntax_Syntax.modul Prims.option = (fun env path -> (match ((FStar_List.tryFind (fun _50_284 -> (match (_50_284) with
 | (mlid, modul) -> begin
 ((FStar_Ident.path_of_lid mlid) = path)
 end)) env.modules)) with
-| Some (_50_285, modul) -> begin
+| Some (_50_286, modul) -> begin
 Some (modul)
 end
 | None -> begin
@@ -378,14 +378,14 @@ let try_lookup_let : env  ->  FStar_Ident.lident  ->  FStar_Syntax_Syntax.term P
 # 248 "FStar.Parser.Env.fst"
 let find_in_sig = (fun lid -> (match ((let _131_213 = (sigmap env)
 in (FStar_Util.smap_try_find _131_213 lid.FStar_Ident.str))) with
-| Some (FStar_Syntax_Syntax.Sig_let ((_50_295, lbs), _50_299, _50_301, _50_303), _50_307) -> begin
+| Some (FStar_Syntax_Syntax.Sig_let ((_50_296, lbs), _50_300, _50_302, _50_304), _50_308) -> begin
 (
 # 251 "FStar.Parser.Env.fst"
 let fv = (lb_fv lbs lid)
 in (let _131_214 = (FStar_Syntax_Syntax.fvar lid fv.FStar_Syntax_Syntax.fv_delta fv.FStar_Syntax_Syntax.fv_qual)
 in Some (_131_214)))
 end
-| _50_312 -> begin
+| _50_313 -> begin
 None
 end))
 in (resolve_in_open_namespaces env lid find_in_sig)))
@@ -395,16 +395,16 @@ let try_lookup_definition : env  ->  FStar_Ident.lident  ->  FStar_Syntax_Syntax
 # 257 "FStar.Parser.Env.fst"
 let find_in_sig = (fun lid -> (match ((let _131_221 = (sigmap env)
 in (FStar_Util.smap_try_find _131_221 lid.FStar_Ident.str))) with
-| Some (FStar_Syntax_Syntax.Sig_let (lbs, _50_319, _50_321, _50_323), _50_327) -> begin
+| Some (FStar_Syntax_Syntax.Sig_let (lbs, _50_320, _50_322, _50_324), _50_328) -> begin
 (FStar_Util.find_map (Prims.snd lbs) (fun lb -> (match (lb.FStar_Syntax_Syntax.lbname) with
 | FStar_Util.Inr (fv) when (FStar_Syntax_Syntax.fv_eq_lid fv lid) -> begin
 Some (lb.FStar_Syntax_Syntax.lbdef)
 end
-| _50_334 -> begin
+| _50_335 -> begin
 None
 end)))
 end
-| _50_336 -> begin
+| _50_337 -> begin
 None
 end))
 in (resolve_in_open_namespaces env lid find_in_sig)))
@@ -414,7 +414,7 @@ let try_lookup_lid' : Prims.bool  ->  Prims.bool  ->  env  ->  FStar_Ident.liden
 | Some (Term_name (e)) -> begin
 Some (e)
 end
-| _50_345 -> begin
+| _50_346 -> begin
 None
 end))
 
@@ -426,12 +426,12 @@ let try_lookup_datacon : env  ->  FStar_Ident.lident  ->  FStar_Syntax_Syntax.fv
 # 276 "FStar.Parser.Env.fst"
 let find_in_sig = (fun lid -> (match ((let _131_241 = (sigmap env)
 in (FStar_Util.smap_try_find _131_241 lid.FStar_Ident.str))) with
-| Some (FStar_Syntax_Syntax.Sig_declare_typ (_50_353, _50_355, _50_357, quals, _50_360), _50_364) -> begin
+| Some (FStar_Syntax_Syntax.Sig_declare_typ (_50_354, _50_356, _50_358, quals, _50_361), _50_365) -> begin
 if (FStar_All.pipe_right quals (FStar_Util.for_some (fun _50_5 -> (match (_50_5) with
 | FStar_Syntax_Syntax.Assumption -> begin
 true
 end
-| _50_370 -> begin
+| _50_371 -> begin
 false
 end)))) then begin
 (let _131_243 = (FStar_Syntax_Syntax.lid_as_fv lid FStar_Syntax_Syntax.Delta_constant None)
@@ -440,11 +440,11 @@ end else begin
 None
 end
 end
-| Some (FStar_Syntax_Syntax.Sig_datacon (_50_372), _50_375) -> begin
+| Some (FStar_Syntax_Syntax.Sig_datacon (_50_373), _50_376) -> begin
 (let _131_244 = (FStar_Syntax_Syntax.lid_as_fv lid FStar_Syntax_Syntax.Delta_constant (Some (FStar_Syntax_Syntax.Data_ctor)))
 in Some (_131_244))
 end
-| _50_379 -> begin
+| _50_380 -> begin
 None
 end))
 in (resolve_in_open_namespaces env lid find_in_sig)))
@@ -454,10 +454,10 @@ let find_all_datacons : env  ->  FStar_Ident.lident  ->  FStar_Ident.lident Prim
 # 287 "FStar.Parser.Env.fst"
 let find_in_sig = (fun lid -> (match ((let _131_251 = (sigmap env)
 in (FStar_Util.smap_try_find _131_251 lid.FStar_Ident.str))) with
-| Some (FStar_Syntax_Syntax.Sig_inductive_typ (_50_385, _50_387, _50_389, _50_391, _50_393, datas, _50_396, _50_398), _50_402) -> begin
+| Some (FStar_Syntax_Syntax.Sig_inductive_typ (_50_386, _50_388, _50_390, _50_392, _50_394, datas, _50_397, _50_399), _50_403) -> begin
 Some (datas)
 end
-| _50_406 -> begin
+| _50_407 -> begin
 None
 end))
 in (resolve_in_open_namespaces env lid find_in_sig)))
@@ -468,7 +468,7 @@ let record_cache_aux : ((Prims.unit  ->  Prims.unit) * (Prims.unit  ->  Prims.un
 let record_cache = (FStar_Util.mk_ref (([])::[]))
 in (
 # 296 "FStar.Parser.Env.fst"
-let push = (fun _50_409 -> (match (()) with
+let push = (fun _50_410 -> (match (()) with
 | () -> begin
 (let _131_265 = (let _131_264 = (let _131_262 = (FStar_ST.read record_cache)
 in (FStar_List.hd _131_262))
@@ -478,7 +478,7 @@ in (FStar_ST.op_Colon_Equals record_cache _131_265))
 end))
 in (
 # 298 "FStar.Parser.Env.fst"
-let pop = (fun _50_411 -> (match (()) with
+let pop = (fun _50_412 -> (match (()) with
 | () -> begin
 (let _131_269 = (let _131_268 = (FStar_ST.read record_cache)
 in (FStar_List.tl _131_268))
@@ -486,7 +486,7 @@ in (FStar_ST.op_Colon_Equals record_cache _131_269))
 end))
 in (
 # 300 "FStar.Parser.Env.fst"
-let peek = (fun _50_413 -> (match (()) with
+let peek = (fun _50_414 -> (match (()) with
 | () -> begin
 (let _131_272 = (FStar_ST.read record_cache)
 in (FStar_List.hd _131_272))
@@ -504,76 +504,76 @@ in (push, pop, peek, insert))))))
 # 304 "FStar.Parser.Env.fst"
 let push_record_cache : Prims.unit  ->  Prims.unit = (
 # 305 "FStar.Parser.Env.fst"
-let _50_423 = record_cache_aux
-in (match (_50_423) with
-| (push, _50_418, _50_420, _50_422) -> begin
+let _50_424 = record_cache_aux
+in (match (_50_424) with
+| (push, _50_419, _50_421, _50_423) -> begin
 push
 end))
 
 # 308 "FStar.Parser.Env.fst"
 let pop_record_cache : Prims.unit  ->  Prims.unit = (
 # 309 "FStar.Parser.Env.fst"
-let _50_431 = record_cache_aux
-in (match (_50_431) with
-| (_50_425, pop, _50_428, _50_430) -> begin
+let _50_432 = record_cache_aux
+in (match (_50_432) with
+| (_50_426, pop, _50_429, _50_431) -> begin
 pop
 end))
 
 # 312 "FStar.Parser.Env.fst"
 let peek_record_cache : Prims.unit  ->  record_or_dc Prims.list = (
 # 313 "FStar.Parser.Env.fst"
-let _50_439 = record_cache_aux
-in (match (_50_439) with
-| (_50_433, _50_435, peek, _50_438) -> begin
+let _50_440 = record_cache_aux
+in (match (_50_440) with
+| (_50_434, _50_436, peek, _50_439) -> begin
 peek
 end))
 
 # 316 "FStar.Parser.Env.fst"
 let insert_record_cache : record_or_dc  ->  Prims.unit = (
 # 317 "FStar.Parser.Env.fst"
-let _50_447 = record_cache_aux
-in (match (_50_447) with
-| (_50_441, _50_443, _50_445, insert) -> begin
+let _50_448 = record_cache_aux
+in (match (_50_448) with
+| (_50_442, _50_444, _50_446, insert) -> begin
 insert
 end))
 
 # 320 "FStar.Parser.Env.fst"
 let extract_record : env  ->  FStar_Syntax_Syntax.sigelt  ->  Prims.unit = (fun e _50_9 -> (match (_50_9) with
-| FStar_Syntax_Syntax.Sig_bundle (sigs, _50_452, _50_454, _50_456) -> begin
+| FStar_Syntax_Syntax.Sig_bundle (sigs, _50_453, _50_455, _50_457) -> begin
 (
 # 322 "FStar.Parser.Env.fst"
 let is_rec = (FStar_Util.for_some (fun _50_6 -> (match (_50_6) with
 | (FStar_Syntax_Syntax.RecordType (_)) | (FStar_Syntax_Syntax.RecordConstructor (_)) -> begin
 true
 end
-| _50_467 -> begin
+| _50_468 -> begin
 false
 end)))
 in (
 # 327 "FStar.Parser.Env.fst"
 let find_dc = (fun dc -> (FStar_All.pipe_right sigs (FStar_Util.find_opt (fun _50_7 -> (match (_50_7) with
-| FStar_Syntax_Syntax.Sig_datacon (lid, _50_474, _50_476, _50_478, _50_480, _50_482, _50_484, _50_486) -> begin
+| FStar_Syntax_Syntax.Sig_datacon (lid, _50_475, _50_477, _50_479, _50_481, _50_483, _50_485, _50_487) -> begin
 (FStar_Ident.lid_equals dc lid)
 end
-| _50_490 -> begin
+| _50_491 -> begin
 false
 end)))))
 in (FStar_All.pipe_right sigs (FStar_List.iter (fun _50_8 -> (match (_50_8) with
-| FStar_Syntax_Syntax.Sig_inductive_typ (typename, univs, parms, _50_496, _50_498, dc::[], tags, _50_503) -> begin
+| FStar_Syntax_Syntax.Sig_inductive_typ (typename, univs, parms, _50_497, _50_499, dc::[], tags, _50_504) -> begin
 (match ((let _131_350 = (find_dc dc)
 in (FStar_All.pipe_left FStar_Util.must _131_350))) with
-| FStar_Syntax_Syntax.Sig_datacon (constrname, _50_508, t, _50_511, _50_513, _50_515, _50_517, _50_519) -> begin
+| FStar_Syntax_Syntax.Sig_datacon (constrname, _50_509, t, _50_512, _50_514, _50_516, _50_518, _50_520) -> begin
 (
 # 336 "FStar.Parser.Env.fst"
-let _50_525 = (FStar_Syntax_Util.arrow_formals t)
-in (match (_50_525) with
-| (formals, _50_524) -> begin
+let _50_526 = (FStar_Syntax_Util.arrow_formals t)
+in (match (_50_526) with
+| (formals, _50_525) -> begin
 (
 # 337 "FStar.Parser.Env.fst"
 let is_rec = (is_rec tags)
 in (
 # 338 "FStar.Parser.Env.fst"
-let fields = (FStar_All.pipe_right formals (FStar_List.collect (fun _50_529 -> (match (_50_529) with
+let fields = (FStar_All.pipe_right formals (FStar_List.collect (fun _50_530 -> (match (_50_530) with
 | (x, q) -> begin
 if ((FStar_Syntax_Syntax.is_null_bv x) || (is_rec && (FStar_Syntax_Syntax.is_implicit q))) then begin
 []
@@ -594,15 +594,15 @@ let record = {typename = typename; constrname = constrname; parms = parms; field
 in (insert_record_cache record))))
 end))
 end
-| _50_533 -> begin
+| _50_534 -> begin
 ()
 end)
 end
-| _50_535 -> begin
+| _50_536 -> begin
 ()
 end))))))
 end
-| _50_537 -> begin
+| _50_538 -> begin
 ()
 end))
 
@@ -631,8 +631,8 @@ in (
 # 362 "FStar.Parser.Env.fst"
 let find_in_cache = (fun fieldname -> (
 # 364 "FStar.Parser.Env.fst"
-let _50_555 = (fieldname.FStar_Ident.ns, fieldname.FStar_Ident.ident)
-in (match (_50_555) with
+let _50_556 = (fieldname.FStar_Ident.ns, fieldname.FStar_Ident.ident)
+in (match (_50_556) with
 | (ns, fieldname) -> begin
 (let _131_370 = (peek_record_cache ())
 in (FStar_Util.find_map _131_370 (fun record -> (
@@ -644,8 +644,8 @@ let ns = (maybe_add_constrname ns constrname)
 in (
 # 368 "FStar.Parser.Env.fst"
 let fname = (FStar_Ident.lid_of_ids (FStar_List.append ns ((fieldname)::[])))
-in (FStar_Util.find_map record.fields (fun _50_563 -> (match (_50_563) with
-| (f, _50_562) -> begin
+in (FStar_Util.find_map record.fields (fun _50_564 -> (match (_50_564) with
+| (f, _50_563) -> begin
 if (FStar_Ident.lid_equals fname f) then begin
 Some ((record, fname))
 end else begin
@@ -660,7 +660,7 @@ let try_lookup_record_by_field_name : env  ->  FStar_Ident.lident  ->  (record_o
 | Some (r, f) when r.is_record -> begin
 Some ((r, f))
 end
-| _50_571 -> begin
+| _50_572 -> begin
 None
 end))
 
@@ -669,7 +669,7 @@ let try_lookup_projector_by_field_name : env  ->  FStar_Ident.lident  ->  (FStar
 | Some (r, f) -> begin
 Some ((f, r.is_record))
 end
-| _50_579 -> begin
+| _50_580 -> begin
 None
 end))
 
@@ -678,8 +678,8 @@ let qualify_field_to_record : env  ->  record_or_dc  ->  FStar_Ident.lident  -> 
 # 386 "FStar.Parser.Env.fst"
 let qualify = (fun fieldname -> (
 # 387 "FStar.Parser.Env.fst"
-let _50_587 = (fieldname.FStar_Ident.ns, fieldname.FStar_Ident.ident)
-in (match (_50_587) with
+let _50_588 = (fieldname.FStar_Ident.ns, fieldname.FStar_Ident.ident)
+in (match (_50_588) with
 | (ns, fieldname) -> begin
 (
 # 388 "FStar.Parser.Env.fst"
@@ -687,8 +687,8 @@ let constrname = recd.constrname.FStar_Ident.ident
 in (
 # 389 "FStar.Parser.Env.fst"
 let fname = (FStar_Ident.lid_of_ids (FStar_List.append (FStar_List.append ns ((constrname)::[])) ((fieldname)::[])))
-in (FStar_Util.find_map recd.fields (fun _50_593 -> (match (_50_593) with
-| (f, _50_592) -> begin
+in (FStar_Util.find_map recd.fields (fun _50_594 -> (match (_50_594) with
+| (f, _50_593) -> begin
 if (FStar_Ident.lid_equals fname f) then begin
 Some (fname)
 end else begin
@@ -703,13 +703,13 @@ let unique : Prims.bool  ->  Prims.bool  ->  env  ->  FStar_Ident.lident  ->  Pr
 # 397 "FStar.Parser.Env.fst"
 let this_env = (
 # 397 "FStar.Parser.Env.fst"
-let _50_598 = env
-in {curmodule = _50_598.curmodule; modules = _50_598.modules; open_namespaces = []; sigaccum = _50_598.sigaccum; localbindings = _50_598.localbindings; recbindings = _50_598.recbindings; sigmap = _50_598.sigmap; default_result_effect = _50_598.default_result_effect; iface = _50_598.iface; admitted_iface = _50_598.admitted_iface; expect_typ = _50_598.expect_typ})
+let _50_599 = env
+in {curmodule = _50_599.curmodule; modules = _50_599.modules; open_namespaces = []; sigaccum = _50_599.sigaccum; localbindings = _50_599.localbindings; recbindings = _50_599.recbindings; sigmap = _50_599.sigmap; default_result_effect = _50_599.default_result_effect; iface = _50_599.iface; admitted_iface = _50_599.admitted_iface; expect_typ = _50_599.expect_typ})
 in (match ((try_lookup_lid' any_val exclude_if env lid)) with
 | None -> begin
 true
 end
-| Some (_50_603) -> begin
+| Some (_50_604) -> begin
 false
 end)))
 
@@ -719,18 +719,18 @@ let push_bv : env  ->  FStar_Ident.ident  ->  (env * FStar_Syntax_Syntax.bv) = (
 let bv = (FStar_Syntax_Syntax.gen_bv x.FStar_Ident.idText (Some (x.FStar_Ident.idRange)) FStar_Syntax_Syntax.tun)
 in ((
 # 404 "FStar.Parser.Env.fst"
-let _50_608 = env
-in {curmodule = _50_608.curmodule; modules = _50_608.modules; open_namespaces = _50_608.open_namespaces; sigaccum = _50_608.sigaccum; localbindings = ((x, bv))::env.localbindings; recbindings = _50_608.recbindings; sigmap = _50_608.sigmap; default_result_effect = _50_608.default_result_effect; iface = _50_608.iface; admitted_iface = _50_608.admitted_iface; expect_typ = _50_608.expect_typ}), bv)))
+let _50_609 = env
+in {curmodule = _50_609.curmodule; modules = _50_609.modules; open_namespaces = _50_609.open_namespaces; sigaccum = _50_609.sigaccum; localbindings = ((x, bv))::env.localbindings; recbindings = _50_609.recbindings; sigmap = _50_609.sigmap; default_result_effect = _50_609.default_result_effect; iface = _50_609.iface; admitted_iface = _50_609.admitted_iface; expect_typ = _50_609.expect_typ}), bv)))
 
 # 406 "FStar.Parser.Env.fst"
-let push_top_level_rec_binding : env  ->  FStar_Ident.ident  ->  env = (fun env x -> (
+let push_top_level_rec_binding : env  ->  FStar_Ident.ident  ->  FStar_Syntax_Syntax.delta_depth  ->  env = (fun env x dd -> (
 # 407 "FStar.Parser.Env.fst"
 let l = (qualify env x)
 in if (unique false true env l) then begin
 (
 # 409 "FStar.Parser.Env.fst"
-let _50_613 = env
-in {curmodule = _50_613.curmodule; modules = _50_613.modules; open_namespaces = _50_613.open_namespaces; sigaccum = _50_613.sigaccum; localbindings = _50_613.localbindings; recbindings = ((x, l))::env.recbindings; sigmap = _50_613.sigmap; default_result_effect = _50_613.default_result_effect; iface = _50_613.iface; admitted_iface = _50_613.admitted_iface; expect_typ = _50_613.expect_typ})
+let _50_615 = env
+in {curmodule = _50_615.curmodule; modules = _50_615.modules; open_namespaces = _50_615.open_namespaces; sigaccum = _50_615.sigaccum; localbindings = _50_615.localbindings; recbindings = ((x, l, dd))::env.recbindings; sigmap = _50_615.sigmap; default_result_effect = _50_615.default_result_effect; iface = _50_615.iface; admitted_iface = _50_615.admitted_iface; expect_typ = _50_615.expect_typ})
 end else begin
 (Prims.raise (FStar_Syntax_Syntax.Error (((Prims.strcat "Duplicate top-level names " l.FStar_Ident.str), (FStar_Ident.range_of_lid l)))))
 end))
@@ -740,14 +740,14 @@ let push_sigelt : env  ->  FStar_Syntax_Syntax.sigelt  ->  env = (fun env s -> (
 # 413 "FStar.Parser.Env.fst"
 let err = (fun l -> (
 # 414 "FStar.Parser.Env.fst"
-let sopt = (let _131_410 = (sigmap env)
-in (FStar_Util.smap_try_find _131_410 l.FStar_Ident.str))
+let sopt = (let _131_412 = (sigmap env)
+in (FStar_Util.smap_try_find _131_412 l.FStar_Ident.str))
 in (
 # 415 "FStar.Parser.Env.fst"
 let r = (match (sopt) with
-| Some (se, _50_622) -> begin
-(match ((let _131_411 = (FStar_Syntax_Util.lids_of_sigelt se)
-in (FStar_Util.find_opt (FStar_Ident.lid_equals l) _131_411))) with
+| Some (se, _50_624) -> begin
+(match ((let _131_413 = (FStar_Syntax_Util.lids_of_sigelt se)
+in (FStar_Util.find_opt (FStar_Ident.lid_equals l) _131_413))) with
 | Some (l) -> begin
 (FStar_All.pipe_left FStar_Range.string_of_range (FStar_Ident.range_of_lid l))
 end
@@ -758,25 +758,25 @@ end
 | None -> begin
 "<unknown>"
 end)
-in (let _131_414 = (let _131_413 = (let _131_412 = (FStar_Util.format2 "Duplicate top-level names [%s]; previously declared at %s" (FStar_Ident.text_of_lid l) r)
-in (_131_412, (FStar_Ident.range_of_lid l)))
-in FStar_Syntax_Syntax.Error (_131_413))
-in (Prims.raise _131_414)))))
+in (let _131_416 = (let _131_415 = (let _131_414 = (FStar_Util.format2 "Duplicate top-level names [%s]; previously declared at %s" (FStar_Ident.text_of_lid l) r)
+in (_131_414, (FStar_Ident.range_of_lid l)))
+in FStar_Syntax_Syntax.Error (_131_415))
+in (Prims.raise _131_416)))))
 in (
 # 423 "FStar.Parser.Env.fst"
 let env = (
 # 424 "FStar.Parser.Env.fst"
-let _50_640 = (match (s) with
-| FStar_Syntax_Syntax.Sig_let (_50_631) -> begin
+let _50_642 = (match (s) with
+| FStar_Syntax_Syntax.Sig_let (_50_633) -> begin
 (false, true)
 end
-| FStar_Syntax_Syntax.Sig_bundle (_50_634) -> begin
+| FStar_Syntax_Syntax.Sig_bundle (_50_636) -> begin
 (true, true)
 end
-| _50_637 -> begin
+| _50_639 -> begin
 (false, false)
 end)
-in (match (_50_640) with
+in (match (_50_642) with
 | (any_val, exclude_if) -> begin
 (
 # 428 "FStar.Parser.Env.fst"
@@ -789,11 +789,11 @@ end))) with
 | None -> begin
 (
 # 430 "FStar.Parser.Env.fst"
-let _50_644 = (extract_record env s)
+let _50_646 = (extract_record env s)
 in (
 # 430 "FStar.Parser.Env.fst"
-let _50_646 = env
-in {curmodule = _50_646.curmodule; modules = _50_646.modules; open_namespaces = _50_646.open_namespaces; sigaccum = (s)::env.sigaccum; localbindings = _50_646.localbindings; recbindings = _50_646.recbindings; sigmap = _50_646.sigmap; default_result_effect = _50_646.default_result_effect; iface = _50_646.iface; admitted_iface = _50_646.admitted_iface; expect_typ = _50_646.expect_typ}))
+let _50_648 = env
+in {curmodule = _50_648.curmodule; modules = _50_648.modules; open_namespaces = _50_648.open_namespaces; sigaccum = (s)::env.sigaccum; localbindings = _50_648.localbindings; recbindings = _50_648.recbindings; sigmap = _50_648.sigmap; default_result_effect = _50_648.default_result_effect; iface = _50_648.iface; admitted_iface = _50_648.admitted_iface; expect_typ = _50_648.expect_typ}))
 end
 | Some (l) -> begin
 (err l)
@@ -801,26 +801,26 @@ end))
 end))
 in (
 # 433 "FStar.Parser.Env.fst"
-let _50_665 = (match (s) with
-| FStar_Syntax_Syntax.Sig_bundle (ses, _50_653, _50_655, _50_657) -> begin
-(let _131_418 = (FStar_List.map (fun se -> (let _131_417 = (FStar_Syntax_Util.lids_of_sigelt se)
-in (_131_417, se))) ses)
-in (env, _131_418))
+let _50_667 = (match (s) with
+| FStar_Syntax_Syntax.Sig_bundle (ses, _50_655, _50_657, _50_659) -> begin
+(let _131_420 = (FStar_List.map (fun se -> (let _131_419 = (FStar_Syntax_Util.lids_of_sigelt se)
+in (_131_419, se))) ses)
+in (env, _131_420))
 end
-| _50_662 -> begin
-(let _131_421 = (let _131_420 = (let _131_419 = (FStar_Syntax_Util.lids_of_sigelt s)
-in (_131_419, s))
-in (_131_420)::[])
-in (env, _131_421))
+| _50_664 -> begin
+(let _131_423 = (let _131_422 = (let _131_421 = (FStar_Syntax_Util.lids_of_sigelt s)
+in (_131_421, s))
+in (_131_422)::[])
+in (env, _131_423))
 end)
-in (match (_50_665) with
+in (match (_50_667) with
 | (env, lss) -> begin
 (
 # 436 "FStar.Parser.Env.fst"
-let _50_670 = (FStar_All.pipe_right lss (FStar_List.iter (fun _50_668 -> (match (_50_668) with
+let _50_672 = (FStar_All.pipe_right lss (FStar_List.iter (fun _50_670 -> (match (_50_670) with
 | (lids, se) -> begin
-(FStar_All.pipe_right lids (FStar_List.iter (fun lid -> (let _131_424 = (sigmap env)
-in (FStar_Util.smap_add _131_424 lid.FStar_Ident.str (se, (env.iface && (not (env.admitted_iface)))))))))
+(FStar_All.pipe_right lids (FStar_List.iter (fun lid -> (let _131_426 = (sigmap env)
+in (FStar_Util.smap_add _131_426 lid.FStar_Ident.str (se, (env.iface && (not (env.admitted_iface)))))))))
 end))))
 in env)
 end)))))
@@ -828,8 +828,8 @@ end)))))
 # 441 "FStar.Parser.Env.fst"
 let push_namespace : env  ->  FStar_Ident.lident  ->  env = (fun env lid -> (
 # 442 "FStar.Parser.Env.fst"
-let _50_674 = env
-in {curmodule = _50_674.curmodule; modules = _50_674.modules; open_namespaces = (lid)::env.open_namespaces; sigaccum = _50_674.sigaccum; localbindings = _50_674.localbindings; recbindings = _50_674.recbindings; sigmap = _50_674.sigmap; default_result_effect = _50_674.default_result_effect; iface = _50_674.iface; admitted_iface = _50_674.admitted_iface; expect_typ = _50_674.expect_typ}))
+let _50_676 = env
+in {curmodule = _50_676.curmodule; modules = _50_676.modules; open_namespaces = (lid)::env.open_namespaces; sigaccum = _50_676.sigaccum; localbindings = _50_676.localbindings; recbindings = _50_676.recbindings; sigmap = _50_676.sigmap; default_result_effect = _50_676.default_result_effect; iface = _50_676.iface; admitted_iface = _50_676.admitted_iface; expect_typ = _50_676.expect_typ}))
 
 # 444 "FStar.Parser.Env.fst"
 let check_admits : env  ->  Prims.unit = (fun env -> (FStar_All.pipe_right env.sigaccum (FStar_List.iter (fun se -> (match (se) with
@@ -838,164 +838,192 @@ let check_admits : env  ->  Prims.unit = (fun env -> (FStar_All.pipe_right env.s
 | None -> begin
 (
 # 449 "FStar.Parser.Env.fst"
-let _50_686 = (let _131_434 = (let _131_433 = (FStar_Range.string_of_range (FStar_Ident.range_of_lid l))
-in (let _131_432 = (FStar_Syntax_Print.lid_to_string l)
-in (FStar_Util.format2 "%s: Warning: Admitting %s without a definition\n" _131_433 _131_432)))
-in (FStar_Util.print_string _131_434))
-in (let _131_435 = (sigmap env)
-in (FStar_Util.smap_add _131_435 l.FStar_Ident.str (FStar_Syntax_Syntax.Sig_declare_typ ((l, u, t, (FStar_Syntax_Syntax.Assumption)::quals, r)), false))))
+let _50_688 = (let _131_436 = (let _131_435 = (FStar_Range.string_of_range (FStar_Ident.range_of_lid l))
+in (let _131_434 = (FStar_Syntax_Print.lid_to_string l)
+in (FStar_Util.format2 "%s: Warning: Admitting %s without a definition\n" _131_435 _131_434)))
+in (FStar_Util.print_string _131_436))
+in (let _131_437 = (sigmap env)
+in (FStar_Util.smap_add _131_437 l.FStar_Ident.str (FStar_Syntax_Syntax.Sig_declare_typ ((l, u, t, (FStar_Syntax_Syntax.Assumption)::quals, r)), false))))
 end
-| Some (_50_689) -> begin
+| Some (_50_691) -> begin
 ()
 end)
 end
-| _50_692 -> begin
+| _50_694 -> begin
 ()
 end)))))
 
 # 455 "FStar.Parser.Env.fst"
 let finish : env  ->  FStar_Syntax_Syntax.modul  ->  env = (fun env modul -> (
 # 456 "FStar.Parser.Env.fst"
-let _50_736 = (FStar_All.pipe_right modul.FStar_Syntax_Syntax.declarations (FStar_List.iter (fun _50_11 -> (match (_50_11) with
-| FStar_Syntax_Syntax.Sig_bundle (ses, quals, _50_699, _50_701) -> begin
-if (FStar_List.contains FStar_Syntax_Syntax.Private quals) then begin
+let _50_754 = (FStar_All.pipe_right modul.FStar_Syntax_Syntax.declarations (FStar_List.iter (fun _50_11 -> (match (_50_11) with
+| FStar_Syntax_Syntax.Sig_bundle (ses, quals, _50_701, _50_703) -> begin
+if ((FStar_List.contains FStar_Syntax_Syntax.Private quals) || (FStar_List.contains FStar_Syntax_Syntax.Abstract quals)) then begin
 (FStar_All.pipe_right ses (FStar_List.iter (fun _50_10 -> (match (_50_10) with
-| FStar_Syntax_Syntax.Sig_datacon (lid, _50_707, _50_709, _50_711, _50_713, _50_715, _50_717, _50_719) -> begin
-(let _131_442 = (sigmap env)
-in (FStar_Util.smap_remove _131_442 lid.FStar_Ident.str))
+| FStar_Syntax_Syntax.Sig_datacon (lid, _50_709, _50_711, _50_713, _50_715, _50_717, _50_719, _50_721) -> begin
+(let _131_444 = (sigmap env)
+in (FStar_Util.smap_remove _131_444 lid.FStar_Ident.str))
 end
-| _50_723 -> begin
+| _50_725 -> begin
 ()
 end))))
 end else begin
 ()
 end
 end
-| FStar_Syntax_Syntax.Sig_declare_typ (lid, _50_726, _50_728, quals, _50_731) -> begin
+| FStar_Syntax_Syntax.Sig_declare_typ (lid, _50_728, _50_730, quals, _50_733) -> begin
 if (FStar_List.contains FStar_Syntax_Syntax.Private quals) then begin
-(let _131_443 = (sigmap env)
-in (FStar_Util.smap_remove _131_443 lid.FStar_Ident.str))
+(let _131_445 = (sigmap env)
+in (FStar_Util.smap_remove _131_445 lid.FStar_Ident.str))
 end else begin
 ()
 end
 end
-| _50_735 -> begin
+| FStar_Syntax_Syntax.Sig_let ((_50_737, lbs), r, _50_742, quals) -> begin
+(
+# 469 "FStar.Parser.Env.fst"
+let _50_747 = if ((FStar_List.contains FStar_Syntax_Syntax.Private quals) || (FStar_List.contains FStar_Syntax_Syntax.Abstract quals)) then begin
+(FStar_All.pipe_right lbs (FStar_List.iter (fun lb -> (let _131_451 = (sigmap env)
+in (let _131_450 = (let _131_449 = (let _131_448 = (let _131_447 = (FStar_Util.right lb.FStar_Syntax_Syntax.lbname)
+in _131_447.FStar_Syntax_Syntax.fv_name)
+in _131_448.FStar_Syntax_Syntax.v)
+in _131_449.FStar_Ident.str)
+in (FStar_Util.smap_remove _131_451 _131_450))))))
+end else begin
+()
+end
+in if (FStar_List.contains FStar_Syntax_Syntax.Abstract quals) then begin
+(FStar_All.pipe_right lbs (FStar_List.iter (fun lb -> (
+# 476 "FStar.Parser.Env.fst"
+let lid = (let _131_454 = (let _131_453 = (FStar_Util.right lb.FStar_Syntax_Syntax.lbname)
+in _131_453.FStar_Syntax_Syntax.fv_name)
+in _131_454.FStar_Syntax_Syntax.v)
+in (
+# 477 "FStar.Parser.Env.fst"
+let decl = FStar_Syntax_Syntax.Sig_declare_typ ((lid, lb.FStar_Syntax_Syntax.lbunivs, lb.FStar_Syntax_Syntax.lbtyp, (FStar_Syntax_Syntax.Assumption)::quals, r))
+in (let _131_455 = (sigmap env)
+in (FStar_Util.smap_add _131_455 lid.FStar_Ident.str (decl, false))))))))
+end else begin
+()
+end)
+end
+| _50_753 -> begin
 ()
 end))))
 in (
-# 466 "FStar.Parser.Env.fst"
-let _50_738 = env
-in {curmodule = None; modules = ((modul.FStar_Syntax_Syntax.name, modul))::env.modules; open_namespaces = []; sigaccum = []; localbindings = []; recbindings = []; sigmap = _50_738.sigmap; default_result_effect = _50_738.default_result_effect; iface = _50_738.iface; admitted_iface = _50_738.admitted_iface; expect_typ = _50_738.expect_typ})))
+# 481 "FStar.Parser.Env.fst"
+let _50_756 = env
+in {curmodule = None; modules = ((modul.FStar_Syntax_Syntax.name, modul))::env.modules; open_namespaces = []; sigaccum = []; localbindings = []; recbindings = []; sigmap = _50_756.sigmap; default_result_effect = _50_756.default_result_effect; iface = _50_756.iface; admitted_iface = _50_756.admitted_iface; expect_typ = _50_756.expect_typ})))
 
-# 474 "FStar.Parser.Env.fst"
+# 489 "FStar.Parser.Env.fst"
 let push : env  ->  env = (fun env -> (
-# 475 "FStar.Parser.Env.fst"
-let _50_741 = (push_record_cache ())
+# 490 "FStar.Parser.Env.fst"
+let _50_759 = (push_record_cache ())
 in (
-# 476 "FStar.Parser.Env.fst"
-let _50_743 = env
-in (let _131_448 = (let _131_447 = (let _131_446 = (sigmap env)
-in (FStar_Util.smap_copy _131_446))
-in (_131_447)::env.sigmap)
-in {curmodule = _50_743.curmodule; modules = _50_743.modules; open_namespaces = _50_743.open_namespaces; sigaccum = _50_743.sigaccum; localbindings = _50_743.localbindings; recbindings = _50_743.recbindings; sigmap = _131_448; default_result_effect = _50_743.default_result_effect; iface = _50_743.iface; admitted_iface = _50_743.admitted_iface; expect_typ = _50_743.expect_typ}))))
+# 491 "FStar.Parser.Env.fst"
+let _50_761 = env
+in (let _131_460 = (let _131_459 = (let _131_458 = (sigmap env)
+in (FStar_Util.smap_copy _131_458))
+in (_131_459)::env.sigmap)
+in {curmodule = _50_761.curmodule; modules = _50_761.modules; open_namespaces = _50_761.open_namespaces; sigaccum = _50_761.sigaccum; localbindings = _50_761.localbindings; recbindings = _50_761.recbindings; sigmap = _131_460; default_result_effect = _50_761.default_result_effect; iface = _50_761.iface; admitted_iface = _50_761.admitted_iface; expect_typ = _50_761.expect_typ}))))
 
-# 479 "FStar.Parser.Env.fst"
+# 494 "FStar.Parser.Env.fst"
 let mark : env  ->  env = (fun env -> (push env))
 
-# 480 "FStar.Parser.Env.fst"
+# 495 "FStar.Parser.Env.fst"
 let reset_mark : env  ->  env = (fun env -> (
-# 480 "FStar.Parser.Env.fst"
-let _50_747 = env
-in (let _131_453 = (FStar_List.tl env.sigmap)
-in {curmodule = _50_747.curmodule; modules = _50_747.modules; open_namespaces = _50_747.open_namespaces; sigaccum = _50_747.sigaccum; localbindings = _50_747.localbindings; recbindings = _50_747.recbindings; sigmap = _131_453; default_result_effect = _50_747.default_result_effect; iface = _50_747.iface; admitted_iface = _50_747.admitted_iface; expect_typ = _50_747.expect_typ})))
+# 495 "FStar.Parser.Env.fst"
+let _50_765 = env
+in (let _131_465 = (FStar_List.tl env.sigmap)
+in {curmodule = _50_765.curmodule; modules = _50_765.modules; open_namespaces = _50_765.open_namespaces; sigaccum = _50_765.sigaccum; localbindings = _50_765.localbindings; recbindings = _50_765.recbindings; sigmap = _131_465; default_result_effect = _50_765.default_result_effect; iface = _50_765.iface; admitted_iface = _50_765.admitted_iface; expect_typ = _50_765.expect_typ})))
 
-# 481 "FStar.Parser.Env.fst"
+# 496 "FStar.Parser.Env.fst"
 let commit_mark : env  ->  env = (fun env -> (match (env.sigmap) with
-| hd::_50_752::tl -> begin
+| hd::_50_770::tl -> begin
 (
-# 482 "FStar.Parser.Env.fst"
-let _50_756 = env
-in {curmodule = _50_756.curmodule; modules = _50_756.modules; open_namespaces = _50_756.open_namespaces; sigaccum = _50_756.sigaccum; localbindings = _50_756.localbindings; recbindings = _50_756.recbindings; sigmap = (hd)::tl; default_result_effect = _50_756.default_result_effect; iface = _50_756.iface; admitted_iface = _50_756.admitted_iface; expect_typ = _50_756.expect_typ})
+# 497 "FStar.Parser.Env.fst"
+let _50_774 = env
+in {curmodule = _50_774.curmodule; modules = _50_774.modules; open_namespaces = _50_774.open_namespaces; sigaccum = _50_774.sigaccum; localbindings = _50_774.localbindings; recbindings = _50_774.recbindings; sigmap = (hd)::tl; default_result_effect = _50_774.default_result_effect; iface = _50_774.iface; admitted_iface = _50_774.admitted_iface; expect_typ = _50_774.expect_typ})
 end
-| _50_759 -> begin
+| _50_777 -> begin
 (FStar_All.failwith "Impossible")
 end))
 
-# 484 "FStar.Parser.Env.fst"
+# 499 "FStar.Parser.Env.fst"
 let pop : env  ->  env = (fun env -> (match (env.sigmap) with
-| _50_763::maps -> begin
+| _50_781::maps -> begin
 (
-# 486 "FStar.Parser.Env.fst"
-let _50_765 = (pop_record_cache ())
+# 501 "FStar.Parser.Env.fst"
+let _50_783 = (pop_record_cache ())
 in (
-# 487 "FStar.Parser.Env.fst"
-let _50_767 = env
-in {curmodule = _50_767.curmodule; modules = _50_767.modules; open_namespaces = _50_767.open_namespaces; sigaccum = _50_767.sigaccum; localbindings = _50_767.localbindings; recbindings = _50_767.recbindings; sigmap = maps; default_result_effect = _50_767.default_result_effect; iface = _50_767.iface; admitted_iface = _50_767.admitted_iface; expect_typ = _50_767.expect_typ}))
+# 502 "FStar.Parser.Env.fst"
+let _50_785 = env
+in {curmodule = _50_785.curmodule; modules = _50_785.modules; open_namespaces = _50_785.open_namespaces; sigaccum = _50_785.sigaccum; localbindings = _50_785.localbindings; recbindings = _50_785.recbindings; sigmap = maps; default_result_effect = _50_785.default_result_effect; iface = _50_785.iface; admitted_iface = _50_785.admitted_iface; expect_typ = _50_785.expect_typ}))
 end
-| _50_770 -> begin
+| _50_788 -> begin
 (FStar_All.failwith "No more modules to pop")
 end))
 
-# 491 "FStar.Parser.Env.fst"
+# 506 "FStar.Parser.Env.fst"
 let export_interface : FStar_Ident.lident  ->  env  ->  env = (fun m env -> (
-# 493 "FStar.Parser.Env.fst"
+# 508 "FStar.Parser.Env.fst"
 let sigelt_in_m = (fun se -> (match ((FStar_Syntax_Util.lids_of_sigelt se)) with
-| l::_50_776 -> begin
+| l::_50_794 -> begin
 (l.FStar_Ident.nsstr = m.FStar_Ident.str)
 end
-| _50_780 -> begin
+| _50_798 -> begin
 false
 end))
 in (
-# 497 "FStar.Parser.Env.fst"
+# 512 "FStar.Parser.Env.fst"
 let sm = (sigmap env)
 in (
-# 498 "FStar.Parser.Env.fst"
+# 513 "FStar.Parser.Env.fst"
 let env = (pop env)
 in (
-# 499 "FStar.Parser.Env.fst"
+# 514 "FStar.Parser.Env.fst"
 let keys = (FStar_Util.smap_keys sm)
 in (
-# 500 "FStar.Parser.Env.fst"
+# 515 "FStar.Parser.Env.fst"
 let sm' = (sigmap env)
 in (
-# 501 "FStar.Parser.Env.fst"
-let _50_804 = (FStar_All.pipe_right keys (FStar_List.iter (fun k -> (match ((FStar_Util.smap_try_find sm' k)) with
+# 516 "FStar.Parser.Env.fst"
+let _50_822 = (FStar_All.pipe_right keys (FStar_List.iter (fun k -> (match ((FStar_Util.smap_try_find sm' k)) with
 | Some (se, true) when (sigelt_in_m se) -> begin
 (
-# 504 "FStar.Parser.Env.fst"
-let _50_790 = (FStar_Util.smap_remove sm' k)
+# 519 "FStar.Parser.Env.fst"
+let _50_808 = (FStar_Util.smap_remove sm' k)
 in (
-# 506 "FStar.Parser.Env.fst"
+# 521 "FStar.Parser.Env.fst"
 let se = (match (se) with
 | FStar_Syntax_Syntax.Sig_declare_typ (l, u, t, q, r) -> begin
 FStar_Syntax_Syntax.Sig_declare_typ ((l, u, t, (FStar_Syntax_Syntax.Assumption)::q, r))
 end
-| _50_800 -> begin
+| _50_818 -> begin
 se
 end)
 in (FStar_Util.smap_add sm' k (se, false))))
 end
-| _50_803 -> begin
+| _50_821 -> begin
 ()
 end))))
 in env)))))))
 
-# 513 "FStar.Parser.Env.fst"
+# 528 "FStar.Parser.Env.fst"
 let finish_module_or_interface : env  ->  FStar_Syntax_Syntax.modul  ->  env = (fun env modul -> (
-# 514 "FStar.Parser.Env.fst"
-let _50_808 = if (not (modul.FStar_Syntax_Syntax.is_interface)) then begin
+# 529 "FStar.Parser.Env.fst"
+let _50_826 = if (not (modul.FStar_Syntax_Syntax.is_interface)) then begin
 (check_admits env)
 end else begin
 ()
 end
 in (finish env modul)))
 
-# 518 "FStar.Parser.Env.fst"
+# 533 "FStar.Parser.Env.fst"
 let prepare_module_or_interface : Prims.bool  ->  Prims.bool  ->  env  ->  FStar_Ident.lident  ->  (env * Prims.bool) = (fun intf admitted env mname -> (
-# 519 "FStar.Parser.Env.fst"
+# 534 "FStar.Parser.Env.fst"
 let prep = (fun env -> (
-# 520 "FStar.Parser.Env.fst"
+# 535 "FStar.Parser.Env.fst"
 let open_ns = if (FStar_Ident.lid_equals mname FStar_Syntax_Const.prims_lid) then begin
 []
 end else begin
@@ -1010,63 +1038,63 @@ end
 end
 end
 in (
-# 524 "FStar.Parser.Env.fst"
-let _50_817 = env
-in {curmodule = Some (mname); modules = _50_817.modules; open_namespaces = open_ns; sigaccum = _50_817.sigaccum; localbindings = _50_817.localbindings; recbindings = _50_817.recbindings; sigmap = env.sigmap; default_result_effect = _50_817.default_result_effect; iface = intf; admitted_iface = admitted; expect_typ = _50_817.expect_typ})))
-in (match ((FStar_All.pipe_right env.modules (FStar_Util.find_opt (fun _50_822 -> (match (_50_822) with
-| (l, _50_821) -> begin
+# 539 "FStar.Parser.Env.fst"
+let _50_835 = env
+in {curmodule = Some (mname); modules = _50_835.modules; open_namespaces = open_ns; sigaccum = _50_835.sigaccum; localbindings = _50_835.localbindings; recbindings = _50_835.recbindings; sigmap = env.sigmap; default_result_effect = _50_835.default_result_effect; iface = intf; admitted_iface = admitted; expect_typ = _50_835.expect_typ})))
+in (match ((FStar_All.pipe_right env.modules (FStar_Util.find_opt (fun _50_840 -> (match (_50_840) with
+| (l, _50_839) -> begin
 (FStar_Ident.lid_equals l mname)
 end))))) with
 | None -> begin
 ((prep env), false)
 end
-| Some (_50_825, m) -> begin
+| Some (_50_843, m) -> begin
 (
-# 529 "FStar.Parser.Env.fst"
-let _50_829 = if ((not (m.FStar_Syntax_Syntax.is_interface)) || intf) then begin
-(let _131_482 = (let _131_481 = (let _131_480 = (FStar_Util.format1 "Duplicate module or interface name: %s" mname.FStar_Ident.str)
-in (_131_480, (FStar_Ident.range_of_lid mname)))
-in FStar_Syntax_Syntax.Error (_131_481))
-in (Prims.raise _131_482))
+# 544 "FStar.Parser.Env.fst"
+let _50_847 = if ((not (m.FStar_Syntax_Syntax.is_interface)) || intf) then begin
+(let _131_494 = (let _131_493 = (let _131_492 = (FStar_Util.format1 "Duplicate module or interface name: %s" mname.FStar_Ident.str)
+in (_131_492, (FStar_Ident.range_of_lid mname)))
+in FStar_Syntax_Syntax.Error (_131_493))
+in (Prims.raise _131_494))
 end else begin
 ()
 end
-in (let _131_484 = (let _131_483 = (push env)
-in (prep _131_483))
-in (_131_484, true)))
+in (let _131_496 = (let _131_495 = (push env)
+in (prep _131_495))
+in (_131_496, true)))
 end)))
 
-# 534 "FStar.Parser.Env.fst"
+# 549 "FStar.Parser.Env.fst"
 let enter_monad_scope : env  ->  FStar_Ident.ident  ->  env = (fun env mname -> (
-# 535 "FStar.Parser.Env.fst"
+# 550 "FStar.Parser.Env.fst"
 let curmod = (current_module env)
 in (
-# 536 "FStar.Parser.Env.fst"
+# 551 "FStar.Parser.Env.fst"
 let mscope = (FStar_Ident.lid_of_ids (FStar_List.append curmod.FStar_Ident.ns ((curmod.FStar_Ident.ident)::(mname)::[])))
 in (
-# 537 "FStar.Parser.Env.fst"
-let _50_835 = env
-in {curmodule = Some (mscope); modules = _50_835.modules; open_namespaces = (curmod)::env.open_namespaces; sigaccum = _50_835.sigaccum; localbindings = _50_835.localbindings; recbindings = _50_835.recbindings; sigmap = _50_835.sigmap; default_result_effect = _50_835.default_result_effect; iface = _50_835.iface; admitted_iface = _50_835.admitted_iface; expect_typ = _50_835.expect_typ}))))
+# 552 "FStar.Parser.Env.fst"
+let _50_853 = env
+in {curmodule = Some (mscope); modules = _50_853.modules; open_namespaces = (curmod)::env.open_namespaces; sigaccum = _50_853.sigaccum; localbindings = _50_853.localbindings; recbindings = _50_853.recbindings; sigmap = _50_853.sigmap; default_result_effect = _50_853.default_result_effect; iface = _50_853.iface; admitted_iface = _50_853.admitted_iface; expect_typ = _50_853.expect_typ}))))
 
-# 541 "FStar.Parser.Env.fst"
+# 556 "FStar.Parser.Env.fst"
 let exit_monad_scope : env  ->  env  ->  env = (fun env0 env -> (
-# 542 "FStar.Parser.Env.fst"
-let _50_839 = env
-in {curmodule = env0.curmodule; modules = _50_839.modules; open_namespaces = env0.open_namespaces; sigaccum = _50_839.sigaccum; localbindings = _50_839.localbindings; recbindings = _50_839.recbindings; sigmap = _50_839.sigmap; default_result_effect = _50_839.default_result_effect; iface = _50_839.iface; admitted_iface = _50_839.admitted_iface; expect_typ = _50_839.expect_typ}))
+# 557 "FStar.Parser.Env.fst"
+let _50_857 = env
+in {curmodule = env0.curmodule; modules = _50_857.modules; open_namespaces = env0.open_namespaces; sigaccum = _50_857.sigaccum; localbindings = _50_857.localbindings; recbindings = _50_857.recbindings; sigmap = _50_857.sigmap; default_result_effect = _50_857.default_result_effect; iface = _50_857.iface; admitted_iface = _50_857.admitted_iface; expect_typ = _50_857.expect_typ}))
 
-# 546 "FStar.Parser.Env.fst"
+# 561 "FStar.Parser.Env.fst"
 let fail_or = (fun lookup lid -> (match ((lookup lid)) with
 | None -> begin
-(let _131_500 = (let _131_499 = (let _131_498 = (FStar_Util.format1 "Identifier not found: [%s]" (FStar_Ident.text_of_lid lid))
-in (_131_498, (FStar_Ident.range_of_lid lid)))
-in FStar_Syntax_Syntax.Error (_131_499))
-in (Prims.raise _131_500))
+(let _131_512 = (let _131_511 = (let _131_510 = (FStar_Util.format1 "Identifier not found: [%s]" (FStar_Ident.text_of_lid lid))
+in (_131_510, (FStar_Ident.range_of_lid lid)))
+in FStar_Syntax_Syntax.Error (_131_511))
+in (Prims.raise _131_512))
 end
 | Some (r) -> begin
 r
 end))
 
-# 551 "FStar.Parser.Env.fst"
+# 566 "FStar.Parser.Env.fst"
 let fail_or2 = (fun lookup id -> (match ((lookup id)) with
 | None -> begin
 (Prims.raise (FStar_Syntax_Syntax.Error (((Prims.strcat (Prims.strcat "Identifier not found [" id.FStar_Ident.idText) "]"), id.FStar_Ident.idRange))))
