src/ocaml-output/FStar_TypeChecker_Env.ml
@@ -950,16 +950,16 @@ let interpreted_symbols : FStar_Ident.lident Prims.list = (FStar_Syntax_Const.op
 let is_interpreted : env  ->  FStar_Syntax_Syntax.term  ->  Prims.bool = (fun env head -> (match ((let _146_662 = (FStar_Syntax_Util.un_uinst head)
 in _146_662.FStar_Syntax_Syntax.n)) with
 | FStar_Syntax_Syntax.Tm_fvar (fv) -> begin
-(FStar_Util.for_some (FStar_Ident.lid_equals fv.FStar_Syntax_Syntax.fv_name.FStar_Syntax_Syntax.v) interpreted_symbols)
+(fv.FStar_Syntax_Syntax.fv_delta = FStar_Syntax_Syntax.Delta_equational)
 end
 | _65_816 -> begin
 false
 end))
 
-# 565 "FStar.TypeChecker.Env.fst"
+# 566 "FStar.TypeChecker.Env.fst"
 let effect_decl_opt : env  ->  FStar_Ident.lident  ->  FStar_Syntax_Syntax.eff_decl Prims.option = (fun env l -> (FStar_All.pipe_right env.effects.decls (FStar_Util.find_opt (fun d -> (FStar_Ident.lid_equals d.FStar_Syntax_Syntax.mname l)))))
 
-# 568 "FStar.TypeChecker.Env.fst"
+# 569 "FStar.TypeChecker.Env.fst"
 let get_effect_decl : env  ->  FStar_Ident.lident  ->  FStar_Syntax_Syntax.eff_decl = (fun env l -> (match ((effect_decl_opt env l)) with
 | None -> begin
 (let _146_674 = (let _146_673 = (let _146_672 = (name_not_found l)
@@ -971,7 +971,7 @@ end
 md
 end))
 
-# 573 "FStar.TypeChecker.Env.fst"
+# 574 "FStar.TypeChecker.Env.fst"
 let join : env  ->  FStar_Ident.lident  ->  FStar_Ident.lident  ->  (FStar_Ident.lident * mlift * mlift) = (fun env l1 l2 -> if (FStar_Ident.lid_equals l1 l2) then begin
 (l1, (fun t wp -> wp), (fun t wp -> wp))
 end else begin
@@ -996,14 +996,14 @@ end)
 end
 end)
 
-# 583 "FStar.TypeChecker.Env.fst"
+# 584 "FStar.TypeChecker.Env.fst"
 let monad_leq : env  ->  FStar_Ident.lident  ->  FStar_Ident.lident  ->  edge Prims.option = (fun env l1 l2 -> if ((FStar_Ident.lid_equals l1 l2) || ((FStar_Ident.lid_equals l1 FStar_Syntax_Const.effect_Tot_lid) && (FStar_Ident.lid_equals l2 FStar_Syntax_Const.effect_GTot_lid))) then begin
 Some ({msource = l1; mtarget = l2; mlift = (fun t wp -> wp)})
 end else begin
 (FStar_All.pipe_right env.effects.order (FStar_Util.find_opt (fun e -> ((FStar_Ident.lid_equals l1 e.msource) && (FStar_Ident.lid_equals l2 e.mtarget)))))
 end)
 
-# 589 "FStar.TypeChecker.Env.fst"
+# 590 "FStar.TypeChecker.Env.fst"
 let wp_sig_aux : FStar_Syntax_Syntax.eff_decl Prims.list  ->  FStar_Ident.lident  ->  (FStar_Syntax_Syntax.bv * FStar_Syntax_Syntax.term) = (fun decls m -> (match ((FStar_All.pipe_right decls (FStar_Util.find_opt (fun d -> (FStar_Ident.lid_equals d.FStar_Syntax_Syntax.mname m))))) with
 | None -> begin
 (let _146_765 = (FStar_Util.format1 "Impossible: declaration for monad %s not found" m.FStar_Ident.str)
@@ -1011,12 +1011,12 @@ in (FStar_All.failwith _146_765))
 end
 | Some (md) -> begin
 (
-# 593 "FStar.TypeChecker.Env.fst"
+# 594 "FStar.TypeChecker.Env.fst"
 let _65_870 = (inst_tscheme (md.FStar_Syntax_Syntax.univs, md.FStar_Syntax_Syntax.signature))
 in (match (_65_870) with
 | (_65_868, s) -> begin
 (
-# 594 "FStar.TypeChecker.Env.fst"
+# 595 "FStar.TypeChecker.Env.fst"
 let s = (FStar_Syntax_Subst.compress s)
 in (match ((md.FStar_Syntax_Syntax.binders, s.FStar_Syntax_Syntax.n)) with
 | ([], FStar_Syntax_Syntax.Tm_arrow ((a, _65_883)::(wp, _65_879)::(wlp, _65_875)::[], c)) when (FStar_Syntax_Syntax.is_teff (FStar_Syntax_Util.comp_result c)) -> begin
@@ -1028,10 +1028,10 @@ end))
 end))
 end))
 
-# 599 "FStar.TypeChecker.Env.fst"
+# 600 "FStar.TypeChecker.Env.fst"
 let wp_signature : env  ->  FStar_Ident.lident  ->  (FStar_Syntax_Syntax.bv * FStar_Syntax_Syntax.term) = (fun env m -> (wp_sig_aux env.effects.decls m))
 
-# 601 "FStar.TypeChecker.Env.fst"
+# 602 "FStar.TypeChecker.Env.fst"
 let default_effect : env  ->  FStar_Ident.lident  ->  FStar_Ident.lident Prims.option = (fun env l -> (FStar_Util.find_map env.default_effects (fun _65_898 -> (match (_65_898) with
 | (l', m) -> begin
 if (FStar_Ident.lid_equals l l') then begin
@@ -1041,7 +1041,7 @@ None
 end
 end))))
 
-# 603 "FStar.TypeChecker.Env.fst"
+# 604 "FStar.TypeChecker.Env.fst"
 let build_lattice : env  ->  FStar_Syntax_Syntax.sigelt  ->  env = (fun env se -> (match (se) with
 | FStar_Syntax_Syntax.Sig_effect_abbrev (l, _65_903, _65_905, c, quals, r) -> begin
 (match ((FStar_Util.find_map quals (fun _65_9 -> (match (_65_9) with
@@ -1056,32 +1056,32 @@ env
 end
 | Some (e) -> begin
 (
-# 607 "FStar.TypeChecker.Env.fst"
+# 608 "FStar.TypeChecker.Env.fst"
 let _65_919 = env
 in {solver = _65_919.solver; range = _65_919.range; curmodule = _65_919.curmodule; gamma = _65_919.gamma; gamma_cache = _65_919.gamma_cache; modules = _65_919.modules; expected_typ = _65_919.expected_typ; sigtab = _65_919.sigtab; is_pattern = _65_919.is_pattern; instantiate_imp = _65_919.instantiate_imp; effects = _65_919.effects; generalize = _65_919.generalize; letrecs = _65_919.letrecs; top_level = _65_919.top_level; check_uvars = _65_919.check_uvars; use_eq = _65_919.use_eq; is_iface = _65_919.is_iface; admit = _65_919.admit; default_effects = ((e, l))::env.default_effects; type_of = _65_919.type_of; universe_of = _65_919.universe_of; use_bv_sorts = _65_919.use_bv_sorts})
 end)
 end
 | FStar_Syntax_Syntax.Sig_new_effect (ne, _65_923) -> begin
 (
-# 610 "FStar.TypeChecker.Env.fst"
+# 611 "FStar.TypeChecker.Env.fst"
 let effects = (
-# 610 "FStar.TypeChecker.Env.fst"
+# 611 "FStar.TypeChecker.Env.fst"
 let _65_926 = env.effects
 in {decls = (ne)::env.effects.decls; order = _65_926.order; joins = _65_926.joins})
 in (
-# 611 "FStar.TypeChecker.Env.fst"
+# 612 "FStar.TypeChecker.Env.fst"
 let _65_929 = env
 in {solver = _65_929.solver; range = _65_929.range; curmodule = _65_929.curmodule; gamma = _65_929.gamma; gamma_cache = _65_929.gamma_cache; modules = _65_929.modules; expected_typ = _65_929.expected_typ; sigtab = _65_929.sigtab; is_pattern = _65_929.is_pattern; instantiate_imp = _65_929.instantiate_imp; effects = effects; generalize = _65_929.generalize; letrecs = _65_929.letrecs; top_level = _65_929.top_level; check_uvars = _65_929.check_uvars; use_eq = _65_929.use_eq; is_iface = _65_929.is_iface; admit = _65_929.admit; default_effects = _65_929.default_effects; type_of = _65_929.type_of; universe_of = _65_929.universe_of; use_bv_sorts = _65_929.use_bv_sorts}))
 end
 | FStar_Syntax_Syntax.Sig_sub_effect (sub, _65_933) -> begin
 (
-# 614 "FStar.TypeChecker.Env.fst"
+# 615 "FStar.TypeChecker.Env.fst"
 let compose_edges = (fun e1 e2 -> {msource = e1.msource; mtarget = e2.mtarget; mlift = (fun r wp1 -> (let _146_786 = (e1.mlift r wp1)
 in (e2.mlift r _146_786)))})
 in (
-# 619 "FStar.TypeChecker.Env.fst"
-let mk_lift = (fun lift_t r wp1 -> (
 # 620 "FStar.TypeChecker.Env.fst"
+let mk_lift = (fun lift_t r wp1 -> (
+# 621 "FStar.TypeChecker.Env.fst"
 let _65_948 = (inst_tscheme lift_t)
 in (match (_65_948) with
 | (_65_946, lift_t) -> begin
@@ -1094,31 +1094,31 @@ in FStar_Syntax_Syntax.Tm_app (_146_797))
 in (FStar_Syntax_Syntax.mk _146_798 None wp1.FStar_Syntax_Syntax.pos))
 end)))
 in (
-# 623 "FStar.TypeChecker.Env.fst"
+# 624 "FStar.TypeChecker.Env.fst"
 let edge = {msource = sub.FStar_Syntax_Syntax.source; mtarget = sub.FStar_Syntax_Syntax.target; mlift = (mk_lift sub.FStar_Syntax_Syntax.lift)}
 in (
-# 627 "FStar.TypeChecker.Env.fst"
+# 628 "FStar.TypeChecker.Env.fst"
 let id_edge = (fun l -> {msource = sub.FStar_Syntax_Syntax.source; mtarget = sub.FStar_Syntax_Syntax.target; mlift = (fun t wp -> wp)})
 in (
-# 632 "FStar.TypeChecker.Env.fst"
-let print_mlift = (fun l -> (
 # 633 "FStar.TypeChecker.Env.fst"
+let print_mlift = (fun l -> (
+# 634 "FStar.TypeChecker.Env.fst"
 let arg = (let _146_815 = (FStar_Ident.lid_of_path (("ARG")::[]) FStar_Range.dummyRange)
 in (FStar_Syntax_Syntax.lid_as_fv _146_815 FStar_Syntax_Syntax.Delta_constant None))
 in (
-# 634 "FStar.TypeChecker.Env.fst"
+# 635 "FStar.TypeChecker.Env.fst"
 let wp = (let _146_816 = (FStar_Ident.lid_of_path (("WP")::[]) FStar_Range.dummyRange)
 in (FStar_Syntax_Syntax.lid_as_fv _146_816 FStar_Syntax_Syntax.Delta_constant None))
 in (let _146_817 = (l arg wp)
 in (FStar_Syntax_Print.term_to_string _146_817)))))
 in (
-# 636 "FStar.TypeChecker.Env.fst"
+# 637 "FStar.TypeChecker.Env.fst"
 let order = (edge)::env.effects.order
 in (
-# 638 "FStar.TypeChecker.Env.fst"
+# 639 "FStar.TypeChecker.Env.fst"
 let ms = (FStar_All.pipe_right env.effects.decls (FStar_List.map (fun e -> e.FStar_Syntax_Syntax.mname)))
 in (
-# 640 "FStar.TypeChecker.Env.fst"
+# 641 "FStar.TypeChecker.Env.fst"
 let find_edge = (fun order _65_965 -> (match (_65_965) with
 | (i, j) -> begin
 if (FStar_Ident.lid_equals i j) then begin
@@ -1128,7 +1128,7 @@ end else begin
 end
 end))
 in (
-# 649 "FStar.TypeChecker.Env.fst"
+# 650 "FStar.TypeChecker.Env.fst"
 let order = (FStar_All.pipe_right ms (FStar_List.fold_left (fun order k -> (let _146_831 = (FStar_All.pipe_right ms (FStar_List.collect (fun i -> if (FStar_Ident.lid_equals i k) then begin
 []
 end else begin
@@ -1148,12 +1148,12 @@ end)))
 end)))
 in (FStar_List.append order _146_831))) order))
 in (
-# 660 "FStar.TypeChecker.Env.fst"
+# 661 "FStar.TypeChecker.Env.fst"
 let order = (FStar_Util.remove_dups (fun e1 e2 -> ((FStar_Ident.lid_equals e1.msource e2.msource) && (FStar_Ident.lid_equals e1.mtarget e2.mtarget))) order)
 in (
-# 662 "FStar.TypeChecker.Env.fst"
+# 663 "FStar.TypeChecker.Env.fst"
 let joins = (FStar_All.pipe_right ms (FStar_List.collect (fun i -> (FStar_All.pipe_right ms (FStar_List.collect (fun j -> (
-# 665 "FStar.TypeChecker.Env.fst"
+# 666 "FStar.TypeChecker.Env.fst"
 let join_opt = (FStar_All.pipe_right ms (FStar_List.fold_left (fun bopt k -> (match ((let _146_923 = (find_edge order (i, k))
 in (let _146_922 = (find_edge order (j, k))
 in (_146_923, _146_922)))) with
@@ -1183,13 +1183,13 @@ end
 ((i, j, k, e1.mlift, e2.mlift))::[]
 end))))))))
 in (
-# 682 "FStar.TypeChecker.Env.fst"
+# 683 "FStar.TypeChecker.Env.fst"
 let effects = (
-# 682 "FStar.TypeChecker.Env.fst"
+# 683 "FStar.TypeChecker.Env.fst"
 let _65_1009 = env.effects
 in {decls = _65_1009.decls; order = order; joins = joins})
 in (
-# 685 "FStar.TypeChecker.Env.fst"
+# 686 "FStar.TypeChecker.Env.fst"
 let _65_1012 = env
 in {solver = _65_1012.solver; range = _65_1012.range; curmodule = _65_1012.curmodule; gamma = _65_1012.gamma; gamma_cache = _65_1012.gamma_cache; modules = _65_1012.modules; expected_typ = _65_1012.expected_typ; sigtab = _65_1012.sigtab; is_pattern = _65_1012.is_pattern; instantiate_imp = _65_1012.instantiate_imp; effects = effects; generalize = _65_1012.generalize; letrecs = _65_1012.letrecs; top_level = _65_1012.top_level; check_uvars = _65_1012.check_uvars; use_eq = _65_1012.use_eq; is_iface = _65_1012.is_iface; admit = _65_1012.admit; default_effects = _65_1012.default_effects; type_of = _65_1012.type_of; universe_of = _65_1012.universe_of; use_bv_sorts = _65_1012.use_bv_sorts})))))))))))))
 end
@@ -1197,9 +1197,9 @@ end
 env
 end))
 
-# 692 "FStar.TypeChecker.Env.fst"
+# 693 "FStar.TypeChecker.Env.fst"
 let push_sigelt : env  ->  FStar_Syntax_Syntax.sigelt  ->  env = (fun env s -> (let _146_974 = (
-# 692 "FStar.TypeChecker.Env.fst"
+# 693 "FStar.TypeChecker.Env.fst"
 let _65_1018 = env
 in (let _146_973 = (let _146_972 = (let _146_971 = (let _146_970 = (FStar_Syntax_Util.lids_of_sigelt s)
 in (_146_970, s))
@@ -1208,9 +1208,9 @@ in (_146_972)::env.gamma)
 in {solver = _65_1018.solver; range = _65_1018.range; curmodule = _65_1018.curmodule; gamma = _146_973; gamma_cache = _65_1018.gamma_cache; modules = _65_1018.modules; expected_typ = _65_1018.expected_typ; sigtab = _65_1018.sigtab; is_pattern = _65_1018.is_pattern; instantiate_imp = _65_1018.instantiate_imp; effects = _65_1018.effects; generalize = _65_1018.generalize; letrecs = _65_1018.letrecs; top_level = _65_1018.top_level; check_uvars = _65_1018.check_uvars; use_eq = _65_1018.use_eq; is_iface = _65_1018.is_iface; admit = _65_1018.admit; default_effects = _65_1018.default_effects; type_of = _65_1018.type_of; universe_of = _65_1018.universe_of; use_bv_sorts = _65_1018.use_bv_sorts}))
 in (build_lattice _146_974 s)))
 
-# 694 "FStar.TypeChecker.Env.fst"
+# 695 "FStar.TypeChecker.Env.fst"
 let push_sigelt_inst : env  ->  FStar_Syntax_Syntax.sigelt  ->  FStar_Syntax_Syntax.universes  ->  env = (fun env s us -> (let _146_985 = (
-# 694 "FStar.TypeChecker.Env.fst"
+# 695 "FStar.TypeChecker.Env.fst"
 let _65_1023 = env
 in (let _146_984 = (let _146_983 = (let _146_982 = (let _146_981 = (FStar_Syntax_Util.lids_of_sigelt s)
 in (_146_981, s, us))
@@ -1219,31 +1219,31 @@ in (_146_983)::env.gamma)
 in {solver = _65_1023.solver; range = _65_1023.range; curmodule = _65_1023.curmodule; gamma = _146_984; gamma_cache = _65_1023.gamma_cache; modules = _65_1023.modules; expected_typ = _65_1023.expected_typ; sigtab = _65_1023.sigtab; is_pattern = _65_1023.is_pattern; instantiate_imp = _65_1023.instantiate_imp; effects = _65_1023.effects; generalize = _65_1023.generalize; letrecs = _65_1023.letrecs; top_level = _65_1023.top_level; check_uvars = _65_1023.check_uvars; use_eq = _65_1023.use_eq; is_iface = _65_1023.is_iface; admit = _65_1023.admit; default_effects = _65_1023.default_effects; type_of = _65_1023.type_of; universe_of = _65_1023.universe_of; use_bv_sorts = _65_1023.use_bv_sorts}))
 in (build_lattice _146_985 s)))
 
-# 696 "FStar.TypeChecker.Env.fst"
+# 697 "FStar.TypeChecker.Env.fst"
 let push_local_binding : env  ->  binding  ->  env = (fun env b -> (
-# 696 "FStar.TypeChecker.Env.fst"
+# 697 "FStar.TypeChecker.Env.fst"
 let _65_1027 = env
 in {solver = _65_1027.solver; range = _65_1027.range; curmodule = _65_1027.curmodule; gamma = (b)::env.gamma; gamma_cache = _65_1027.gamma_cache; modules = _65_1027.modules; expected_typ = _65_1027.expected_typ; sigtab = _65_1027.sigtab; is_pattern = _65_1027.is_pattern; instantiate_imp = _65_1027.instantiate_imp; effects = _65_1027.effects; generalize = _65_1027.generalize; letrecs = _65_1027.letrecs; top_level = _65_1027.top_level; check_uvars = _65_1027.check_uvars; use_eq = _65_1027.use_eq; is_iface = _65_1027.is_iface; admit = _65_1027.admit; default_effects = _65_1027.default_effects; type_of = _65_1027.type_of; universe_of = _65_1027.universe_of; use_bv_sorts = _65_1027.use_bv_sorts}))
 
-# 698 "FStar.TypeChecker.Env.fst"
+# 699 "FStar.TypeChecker.Env.fst"
 let push_bv : env  ->  FStar_Syntax_Syntax.bv  ->  env = (fun env x -> (push_local_binding env (Binding_var (x))))
 
-# 700 "FStar.TypeChecker.Env.fst"
+# 701 "FStar.TypeChecker.Env.fst"
 let push_binders : env  ->  FStar_Syntax_Syntax.binders  ->  env = (fun env bs -> (FStar_List.fold_left (fun env _65_1037 -> (match (_65_1037) with
 | (x, _65_1036) -> begin
 (push_bv env x)
 end)) env bs))
 
-# 703 "FStar.TypeChecker.Env.fst"
+# 704 "FStar.TypeChecker.Env.fst"
 let binding_of_lb : FStar_Syntax_Syntax.lbname  ->  (FStar_Ident.ident Prims.list * FStar_Syntax_Syntax.term)  ->  binding = (fun x t -> (match (x) with
 | FStar_Util.Inl (x) -> begin
 (
-# 705 "FStar.TypeChecker.Env.fst"
+# 706 "FStar.TypeChecker.Env.fst"
 let _65_1042 = ()
 in (
-# 706 "FStar.TypeChecker.Env.fst"
+# 707 "FStar.TypeChecker.Env.fst"
 let x = (
-# 706 "FStar.TypeChecker.Env.fst"
+# 707 "FStar.TypeChecker.Env.fst"
 let _65_1044 = x
 in {FStar_Syntax_Syntax.ppname = _65_1044.FStar_Syntax_Syntax.ppname; FStar_Syntax_Syntax.index = _65_1044.FStar_Syntax_Syntax.index; FStar_Syntax_Syntax.sort = (Prims.snd t)})
 in Binding_var (x)))
@@ -1252,28 +1252,28 @@ end
 Binding_lid ((fv.FStar_Syntax_Syntax.fv_name.FStar_Syntax_Syntax.v, t))
 end))
 
-# 711 "FStar.TypeChecker.Env.fst"
+# 712 "FStar.TypeChecker.Env.fst"
 let push_let_binding : env  ->  FStar_Syntax_Syntax.lbname  ->  FStar_Syntax_Syntax.tscheme  ->  env = (fun env lb ts -> (push_local_binding env (binding_of_lb lb ts)))
 
-# 713 "FStar.TypeChecker.Env.fst"
-let push_module : env  ->  FStar_Syntax_Syntax.modul  ->  env = (fun env m -> (
 # 714 "FStar.TypeChecker.Env.fst"
+let push_module : env  ->  FStar_Syntax_Syntax.modul  ->  env = (fun env m -> (
+# 715 "FStar.TypeChecker.Env.fst"
 let _65_1054 = (add_sigelts env m.FStar_Syntax_Syntax.exports)
 in (
-# 715 "FStar.TypeChecker.Env.fst"
+# 716 "FStar.TypeChecker.Env.fst"
 let _65_1056 = env
 in {solver = _65_1056.solver; range = _65_1056.range; curmodule = _65_1056.curmodule; gamma = []; gamma_cache = _65_1056.gamma_cache; modules = (m)::env.modules; expected_typ = None; sigtab = _65_1056.sigtab; is_pattern = _65_1056.is_pattern; instantiate_imp = _65_1056.instantiate_imp; effects = _65_1056.effects; generalize = _65_1056.generalize; letrecs = _65_1056.letrecs; top_level = _65_1056.top_level; check_uvars = _65_1056.check_uvars; use_eq = _65_1056.use_eq; is_iface = _65_1056.is_iface; admit = _65_1056.admit; default_effects = _65_1056.default_effects; type_of = _65_1056.type_of; universe_of = _65_1056.universe_of; use_bv_sorts = _65_1056.use_bv_sorts})))
 
-# 720 "FStar.TypeChecker.Env.fst"
+# 721 "FStar.TypeChecker.Env.fst"
 let push_univ_vars : env  ->  FStar_Syntax_Syntax.univ_names  ->  env = (fun env xs -> (FStar_List.fold_left (fun env x -> (push_local_binding env (Binding_univ (x)))) env xs))
 
-# 723 "FStar.TypeChecker.Env.fst"
-let set_expected_typ : env  ->  FStar_Syntax_Syntax.typ  ->  env = (fun env t -> (
 # 724 "FStar.TypeChecker.Env.fst"
+let set_expected_typ : env  ->  FStar_Syntax_Syntax.typ  ->  env = (fun env t -> (
+# 725 "FStar.TypeChecker.Env.fst"
 let _65_1064 = env
 in {solver = _65_1064.solver; range = _65_1064.range; curmodule = _65_1064.curmodule; gamma = _65_1064.gamma; gamma_cache = _65_1064.gamma_cache; modules = _65_1064.modules; expected_typ = Some (t); sigtab = _65_1064.sigtab; is_pattern = _65_1064.is_pattern; instantiate_imp = _65_1064.instantiate_imp; effects = _65_1064.effects; generalize = _65_1064.generalize; letrecs = _65_1064.letrecs; top_level = _65_1064.top_level; check_uvars = _65_1064.check_uvars; use_eq = false; is_iface = _65_1064.is_iface; admit = _65_1064.admit; default_effects = _65_1064.default_effects; type_of = _65_1064.type_of; universe_of = _65_1064.universe_of; use_bv_sorts = _65_1064.use_bv_sorts}))
 
-# 726 "FStar.TypeChecker.Env.fst"
+# 727 "FStar.TypeChecker.Env.fst"
 let expected_typ : env  ->  FStar_Syntax_Syntax.typ Prims.option = (fun env -> (match (env.expected_typ) with
 | None -> begin
 None
@@ -1282,19 +1282,19 @@ end
 Some (t)
 end))
 
-# 730 "FStar.TypeChecker.Env.fst"
+# 731 "FStar.TypeChecker.Env.fst"
 let clear_expected_typ : env  ->  (env * FStar_Syntax_Syntax.typ Prims.option) = (fun env -> (let _146_1028 = (expected_typ env)
 in ((
-# 731 "FStar.TypeChecker.Env.fst"
+# 732 "FStar.TypeChecker.Env.fst"
 let _65_1071 = env
 in {solver = _65_1071.solver; range = _65_1071.range; curmodule = _65_1071.curmodule; gamma = _65_1071.gamma; gamma_cache = _65_1071.gamma_cache; modules = _65_1071.modules; expected_typ = None; sigtab = _65_1071.sigtab; is_pattern = _65_1071.is_pattern; instantiate_imp = _65_1071.instantiate_imp; effects = _65_1071.effects; generalize = _65_1071.generalize; letrecs = _65_1071.letrecs; top_level = _65_1071.top_level; check_uvars = _65_1071.check_uvars; use_eq = false; is_iface = _65_1071.is_iface; admit = _65_1071.admit; default_effects = _65_1071.default_effects; type_of = _65_1071.type_of; universe_of = _65_1071.universe_of; use_bv_sorts = _65_1071.use_bv_sorts}), _146_1028)))
 
-# 733 "FStar.TypeChecker.Env.fst"
-let finish_module : env  ->  FStar_Syntax_Syntax.modul  ->  env = (
 # 734 "FStar.TypeChecker.Env.fst"
+let finish_module : env  ->  FStar_Syntax_Syntax.modul  ->  env = (
+# 735 "FStar.TypeChecker.Env.fst"
 let empty_lid = (FStar_Ident.lid_of_ids (((FStar_Ident.id_of_text ""))::[]))
 in (fun env m -> (
-# 736 "FStar.TypeChecker.Env.fst"
+# 737 "FStar.TypeChecker.Env.fst"
 let sigs = if (FStar_Ident.lid_equals m.FStar_Syntax_Syntax.name FStar_Syntax_Const.prims_lid) then begin
 (FStar_All.pipe_right env.gamma (FStar_List.collect (fun _65_10 -> (match (_65_10) with
 | Binding_sig (_65_1078, se) -> begin
@@ -1307,25 +1307,25 @@ end else begin
 m.FStar_Syntax_Syntax.exports
 end
 in (
-# 742 "FStar.TypeChecker.Env.fst"
+# 743 "FStar.TypeChecker.Env.fst"
 let _65_1085 = (add_sigelts env sigs)
 in (
-# 743 "FStar.TypeChecker.Env.fst"
+# 744 "FStar.TypeChecker.Env.fst"
 let _65_1087 = (FStar_Util.smap_clear env.gamma_cache)
 in (
-# 744 "FStar.TypeChecker.Env.fst"
+# 745 "FStar.TypeChecker.Env.fst"
 let _65_1089 = env
 in {solver = _65_1089.solver; range = _65_1089.range; curmodule = empty_lid; gamma = []; gamma_cache = _65_1089.gamma_cache; modules = (m)::env.modules; expected_typ = _65_1089.expected_typ; sigtab = _65_1089.sigtab; is_pattern = _65_1089.is_pattern; instantiate_imp = _65_1089.instantiate_imp; effects = _65_1089.effects; generalize = _65_1089.generalize; letrecs = _65_1089.letrecs; top_level = _65_1089.top_level; check_uvars = _65_1089.check_uvars; use_eq = _65_1089.use_eq; is_iface = _65_1089.is_iface; admit = _65_1089.admit; default_effects = _65_1089.default_effects; type_of = _65_1089.type_of; universe_of = _65_1089.universe_of; use_bv_sorts = _65_1089.use_bv_sorts}))))))
 
-# 752 "FStar.TypeChecker.Env.fst"
-let uvars_in_env : env  ->  FStar_Syntax_Syntax.uvars = (fun env -> (
 # 753 "FStar.TypeChecker.Env.fst"
+let uvars_in_env : env  ->  FStar_Syntax_Syntax.uvars = (fun env -> (
+# 754 "FStar.TypeChecker.Env.fst"
 let no_uvs = (FStar_Syntax_Syntax.new_uv_set ())
 in (
-# 754 "FStar.TypeChecker.Env.fst"
+# 755 "FStar.TypeChecker.Env.fst"
 let ext = (fun out uvs -> (FStar_Util.set_union out uvs))
 in (
-# 755 "FStar.TypeChecker.Env.fst"
+# 756 "FStar.TypeChecker.Env.fst"
 let rec aux = (fun out g -> (match (g) with
 | [] -> begin
 out
@@ -1343,15 +1343,15 @@ out
 end))
 in (aux no_uvs env.gamma)))))
 
-# 764 "FStar.TypeChecker.Env.fst"
-let univ_vars : env  ->  FStar_Syntax_Syntax.universe_uvar FStar_Util.set = (fun env -> (
 # 765 "FStar.TypeChecker.Env.fst"
+let univ_vars : env  ->  FStar_Syntax_Syntax.universe_uvar FStar_Util.set = (fun env -> (
+# 766 "FStar.TypeChecker.Env.fst"
 let no_univs = FStar_Syntax_Syntax.no_universe_uvars
 in (
-# 766 "FStar.TypeChecker.Env.fst"
+# 767 "FStar.TypeChecker.Env.fst"
 let ext = (fun out uvs -> (FStar_Util.set_union out uvs))
 in (
-# 767 "FStar.TypeChecker.Env.fst"
+# 768 "FStar.TypeChecker.Env.fst"
 let rec aux = (fun out g -> (match (g) with
 | [] -> begin
 out
@@ -1369,7 +1369,7 @@ out
 end))
 in (aux no_univs env.gamma)))))
 
-# 776 "FStar.TypeChecker.Env.fst"
+# 777 "FStar.TypeChecker.Env.fst"
 let bound_vars_of_bindings : binding Prims.list  ->  FStar_Syntax_Syntax.bv Prims.list = (fun bs -> (FStar_All.pipe_right bs (FStar_List.collect (fun _65_11 -> (match (_65_11) with
 | Binding_var (x) -> begin
 (x)::[]
@@ -1378,23 +1378,23 @@ end
 []
 end)))))
 
-# 784 "FStar.TypeChecker.Env.fst"
+# 785 "FStar.TypeChecker.Env.fst"
 let binders_of_bindings : binding Prims.list  ->  FStar_Syntax_Syntax.binders = (fun bs -> (let _146_1064 = (let _146_1063 = (bound_vars_of_bindings bs)
 in (FStar_All.pipe_right _146_1063 (FStar_List.map FStar_Syntax_Syntax.mk_binder)))
 in (FStar_All.pipe_right _146_1064 FStar_List.rev)))
 
-# 786 "FStar.TypeChecker.Env.fst"
+# 787 "FStar.TypeChecker.Env.fst"
 let bound_vars : env  ->  FStar_Syntax_Syntax.bv Prims.list = (fun env -> (bound_vars_of_bindings env.gamma))
 
-# 788 "FStar.TypeChecker.Env.fst"
+# 789 "FStar.TypeChecker.Env.fst"
 let all_binders : env  ->  FStar_Syntax_Syntax.binders = (fun env -> (binders_of_bindings env.gamma))
 
-# 790 "FStar.TypeChecker.Env.fst"
+# 791 "FStar.TypeChecker.Env.fst"
 let fold_env = (fun env f a -> (FStar_List.fold_right (fun e a -> (f a e)) env.gamma a))
 
-# 792 "FStar.TypeChecker.Env.fst"
-let lidents : env  ->  FStar_Ident.lident Prims.list = (fun env -> (
 # 793 "FStar.TypeChecker.Env.fst"
+let lidents : env  ->  FStar_Ident.lident Prims.list = (fun env -> (
+# 794 "FStar.TypeChecker.Env.fst"
 let keys = (FStar_List.fold_left (fun keys _65_12 -> (match (_65_12) with
 | Binding_sig (lids, _65_1204) -> begin
 (FStar_List.append lids keys)
@@ -1406,10 +1406,10 @@ in (let _146_1088 = (sigtab env)
 in (FStar_Util.smap_fold _146_1088 (fun _65_1210 v keys -> (let _146_1087 = (FStar_Syntax_Util.lids_of_sigelt v)
 in (FStar_List.append _146_1087 keys))) keys))))
 
-# 800 "FStar.TypeChecker.Env.fst"
+# 801 "FStar.TypeChecker.Env.fst"
 let dummy_solver : solver_t = {init = (fun _65_1214 -> ()); push = (fun _65_1216 -> ()); pop = (fun _65_1218 -> ()); mark = (fun _65_1220 -> ()); reset_mark = (fun _65_1222 -> ()); commit_mark = (fun _65_1224 -> ()); encode_modul = (fun _65_1226 _65_1228 -> ()); encode_sig = (fun _65_1230 _65_1232 -> ()); solve = (fun _65_1234 _65_1236 -> ()); is_trivial = (fun _65_1238 _65_1240 -> false); finish = (fun _65_1242 -> ()); refresh = (fun _65_1243 -> ())}
 
-# 815 "FStar.TypeChecker.Env.fst"
+# 816 "FStar.TypeChecker.Env.fst"
 let no_solver_env : (env  ->  FStar_Syntax_Syntax.term  ->  (FStar_Syntax_Syntax.typ * guard_t))  ->  env = (fun tc -> (let _146_1117 = (FStar_Ident.lid_of_path (("dummy")::[]) FStar_Range.dummyRange)
 in (initial_env tc dummy_solver _146_1117)))
 
