examples/test/test.fst
@@ -1,47 +1,7 @@
+module Test0
+abstract type t (x:int) = int
+
 module Test
-
-type rw =
-  | Reader
-  | Writer
-
-new type id
-new type rid
-new type rref : rid -> Type0 -> Type0
-new type entry : id -> Type0
-new type seq : Type0 -> Type0
-
-type state (i:id) (rw:rw) =
-  | State: #region:rid 
-         -> #peer_region:rid
-         -> log: rref (if rw=Reader then peer_region else region) (seq (entry i)) // ghost, subject to cryptographic assumption
-         -> state i rw
-
-type writer i = s:state i Writer
-type reader i = s:state i Reader
-
-// Generate a fresh instance with index i in a fresh sub-region of r0
-// (we might drop this spec, since F* will infer something at least as precise,
-// but we keep it for documentation)
-val gen: reader_parent:rid -> writer_parent:rid -> i:id -> ST (reader i * writer i)
-  (requires (fun h0 -> HyperHeap.disjoint reader_parent writer_parent))
-  (ensures  (fun h0 (rw:reader i * writer i) h1 ->
-           let r = fst rw in 
-           let w = snd rw in 
-           (* let bang = fun x -> sel h1 x in  *)
-           modifies Set.empty h0 h1
-         /\ w.region = r.peer_region
-         /\ r.region = w.peer_region
-         /\ extends (w.region) writer_parent
-         /\ extends (r.region) reader_parent
-         /\ fresh_region w.region h0 h1
-         /\ fresh_region r.region h0 h1
-         /\ op_Equality #(rref w.region (seq (entry i))) w.log r.log  //the explicit annotation here 
-         /\ contains_ref w.counter h1
-         /\ contains_ref r.counter h1
-         /\ contains_ref w.log h1
-         /\ sel h1 w.counter = 0
-         /\ sel h1 r.counter = 0
-         /\ sel h1 w.log = createEmpty
-         ))
-
-
+open Test0
+abstract type t (x:bool) = int
+abstract val foo : t true -> Lemma (requires True) (ensures True) [SMTPatT (t true)]
