ulib/FStar.SeqProperties.fst
@@ -24,27 +24,27 @@ module FStar.SeqProperties
 #set-options "--max_fuel 0 --initial_fuel 0 --initial_ifuel 0 --max_ifuel 0"
 open FStar.Seq
 
-val lemma_append_inj_l: #a:Type -> s1:seq a -> s2:seq a -> t1:seq a -> t2:seq a{length s1 = length t1 /\ Eq (append s1 s2) (append t1 t2)} -> i:nat{i < length s1}
+val lemma_append_inj_l: #a:Type -> s1:seq a -> s2:seq a -> t1:seq a -> t2:seq a{length s1 = length t1 /\ equal (append s1 s2) (append t1 t2)} -> i:nat{i < length s1}
   -> Lemma (index s1 i == index t1 i)
 let lemma_append_inj_l #a s1 s2 t1 t2 i =
   assert (index s1 i = (index (append s1 s2) i));
   assert (index t1 i = (index (append t1 t2) i))
 
-val lemma_append_inj_r: #a:Type -> s1:seq a -> s2:seq a -> t1:seq a -> t2:seq a{length s1 = length t1 /\ length s2 = length t2 /\ Eq (append s1 s2) (append t1 t2)} -> i:nat{i < length s2}
+val lemma_append_inj_r: #a:Type -> s1:seq a -> s2:seq a -> t1:seq a -> t2:seq a{length s1 = length t1 /\ length s2 = length t2 /\ equal (append s1 s2) (append t1 t2)} -> i:nat{i < length s2}
   -> Lemma (ensures  (index s2 i == index t2 i))
 let lemma_append_inj_r #a s1 s2 t1 t2 i =
   assert (index s2 i = (index (append s1 s2) (i + length s1)));
   assert (index t2 i = (index (append t1 t2) (i + length t1)))
 
-val lemma_append_len_disj: #a:Type -> s1:seq a -> s2:seq a -> t1:seq a -> t2:seq a {(length s1 = length t1 \/ length s2 = length t2) /\ (Eq (append s1 s2) (append t1 t2))}
+val lemma_append_len_disj: #a:Type -> s1:seq a -> s2:seq a -> t1:seq a -> t2:seq a {(length s1 = length t1 \/ length s2 = length t2) /\ (equal (append s1 s2) (append t1 t2))}
   -> Lemma (ensures (length s1 = length t1 /\ length s2 = length t2))
 let lemma_append_len_disj #a s1 s2 t1 t2 =
   cut (length (append s1 s2) == length s1 + length s2);
   cut (length (append t1 t2) == length t1 + length t2)
 
 val lemma_append_inj: #a:Type -> s1:seq a -> s2:seq a -> t1:seq a -> t2:seq a {length s1 = length t1 \/ length s2 = length t2}
-  -> Lemma (requires (Eq (append s1 s2) (append t1 t2)))
-           (ensures (Eq s1 t1 /\ Eq s2 t2))
+  -> Lemma (requires (equal (append s1 s2) (append t1 t2)))
+           (ensures (equal s1 t1 /\ equal s2 t2))
 let lemma_append_inj #a s1 s2 t1 t2 =
   lemma_append_len_disj s1 s2 t1 t2;
   Classical.forall_intro #(i:nat{i < length s1}) #(fun i -> index s1 i == index t1 i) (lemma_append_inj_l s1 s2 t1 t2);
@@ -65,7 +65,7 @@ let split #a s i = slice s 0 i, slice s i (length s)
 val lemma_split : #a:Type -> s:seq a -> i:nat{(0 <= i /\ i <= length s)} -> Lemma
   (ensures (append (fst (split s i)) (snd (split s i)) = s))
 let lemma_split #a s i =
-  cut (Eq (append (fst (split s i)) (snd (split s i)))  s)
+  cut (equal (append (fst (split s i)) (snd (split s i)))  s)
 
 val split_eq: #a:Type -> s:seq a -> i:nat{(0 <= i /\ i <= length s)} -> Pure
   (seq a * seq a)
@@ -90,16 +90,16 @@ val swap: #a:Type -> s:seq a -> i:nat{i<length s} -> j:nat{j<length s} -> Tot (s
 let swap #a s i j = upd (upd s j (index s i)) i (index s j)
 
 val lemma_slice_append: #a:Type -> s1:seq a{length s1 >= 1} -> s2:seq a -> Lemma
-  (ensures (Eq (append s1 s2) (append (slice s1 0 1) (append (slice s1 1 (length s1)) s2))))
+  (ensures (equal (append s1 s2) (append (slice s1 0 1) (append (slice s1 1 (length s1)) s2))))
 let lemma_slice_append #a s1 s2 = ()
 
 val lemma_append_cons: #a:Type -> s1:seq a{length s1 > 0} -> s2:seq a -> Lemma
   (requires True)
-  (ensures (Eq (append s1 s2) (cons (head s1) (append (tail s1) s2))))
+  (ensures (equal (append s1 s2) (cons (head s1) (append (tail s1) s2))))
 let rec lemma_append_cons #a s1 s2 = ()
 
 val lemma_tl: #a:Type -> hd:a -> tl:seq a -> Lemma
-  (ensures (Eq (tail (cons hd tl)) tl))
+  (ensures (equal (tail (cons hd tl)) tl))
 let lemma_tl #a hd tl = ()
 
 val sorted: #a:Type
@@ -119,13 +119,13 @@ val lemma_append_count: #a:Type -> lo:seq a -> hi:seq a -> Lemma
   (decreases (length lo))
 let rec lemma_append_count #a lo hi =
   if length lo = 0
-  then cut (Eq (append lo hi) hi)
-  else (cut (Eq (cons (head lo) (append (tail lo) hi))
+  then cut (equal (append lo hi) hi)
+  else (cut (equal (cons (head lo) (append (tail lo) hi))
                 (append lo hi));
         lemma_append_count (tail lo) hi;
         let tl_l_h = append (tail lo) hi in
         let lh = cons (head lo) tl_l_h in
-        cut (Eq (tail lh) tl_l_h))
+        cut (equal (tail lh) tl_l_h))
 
 val lemma_append_count_aux: #a:Type -> x:a -> lo:seq a -> hi:seq a -> Lemma
   (requires True)
@@ -152,7 +152,7 @@ val lemma_count_slice: #a:Type -> s:seq a -> i:nat{i<=length s} -> Lemma
   (ensures (forall x. count x s = count x (slice s 0 i) + count x (slice s i (length s))))
   (decreases (length s))
 let lemma_count_slice #a s i =
-  cut (Eq s (append (slice s 0 i) (slice s i (length s))));
+  cut (equal s (append (slice s 0 i) (slice s i (length s))));
   lemma_append_count (slice s 0 i) (slice s i (length s))
 
 type total_order (a:Type) (f: (a -> a -> Tot bool)) =
@@ -172,8 +172,8 @@ val sorted_concat_lemma: #a:Type
                                (decreases (length lo))
 let rec sorted_concat_lemma #a f lo pivot hi =
   if length lo = 0
-  then (cut (Eq (append lo (cons pivot hi)) (cons pivot hi));
-        cut (Eq (tail (cons pivot hi)) hi))
+  then (cut (equal (append lo (cons pivot hi)) (cons pivot hi));
+        cut (equal (tail (cons pivot hi)) hi))
   else (sorted_concat_lemma f (tail lo) pivot hi;
         lemma_append_cons lo (cons pivot hi);
         lemma_tl (head lo) (append (tail lo) (cons pivot hi)))
@@ -184,11 +184,11 @@ val split_5 : #a:Type -> s:seq a -> i:nat -> j:nat{i < j && j < length s} -> Pur
   (ensures (fun x ->
             ((length x = 5)
              /\ (s = append (index x 0) (append (index x 1) (append (index x 2) (append (index x 3) (index x 4)))))
-             /\ Eq (index x 0) (slice s 0 i)
-             /\ Eq (index x 1) (slice s i (i+1))
-             /\ Eq (index x 2) (slice s (i+1) j)
-             /\ Eq (index x 3) (slice s j (j + 1))
-             /\ Eq (index x 4) (slice s (j + 1) (length s)))))
+             /\ equal (index x 0) (slice s 0 i)
+             /\ equal (index x 1) (slice s i (i+1))
+             /\ equal (index x 2) (slice s (i+1) j)
+             /\ equal (index x 3) (slice s j (j + 1))
+             /\ equal (index x 4) (slice s (j + 1) (length s)))))
 let split_5 #a s i j = admit()
 (* this often fails with Unknown assertion failed *)
 (* let split_5 s i j = *)
@@ -209,9 +209,9 @@ val lemma_swap_permutes_aux_frag_eq: #a:Type -> s:seq a -> i:nat{i<length s} -> 
                                             /\ slice s i (i + 1) = slice (swap s i j) j (j + 1)
                                             /\ slice s j (j + 1) = slice (swap s i j) i (i + 1)))
 let lemma_swap_permutes_aux_frag_eq #a s i j i' j' =
-  cut (Eq (slice s i' j') (slice (swap s i j) i' j'));
-  cut (Eq (slice s i (i + 1))  (slice (swap s i j) j (j + 1)));
-  cut (Eq (slice s j (j + 1))  (slice (swap s i j) i (i + 1)))
+  cut (equal (slice s i' j') (slice (swap s i j) i' j'));
+  cut (equal (slice s i (i + 1))  (slice (swap s i j) j (j + 1)));
+  cut (equal (slice s j (j + 1))  (slice (swap s i j) i (i + 1)))
 
 #set-options "--max_fuel 1 --initial_fuel 1 --initial_ifuel 0 --max_ifuel 0"
 val lemma_swap_permutes_aux: #a:Type -> s:seq a -> i:nat{i<length s} -> j:nat{i <= j && j<length s} -> x:a -> Lemma
@@ -219,7 +219,7 @@ val lemma_swap_permutes_aux: #a:Type -> s:seq a -> i:nat{i<length s} -> j:nat{i 
   (ensures (count x s = count x (swap s i j)))
 let lemma_swap_permutes_aux #a s i j x =
   if j=i
-  then cut (Eq (swap s i j) s)
+  then cut (equal (swap s i j) s)
   else begin
       let s5 = split_5 s i j in
       let frag_lo, frag_i, frag_mid, frag_j, frag_hi =
@@ -266,47 +266,47 @@ let lemma_mem_append #a s1 s2 = lemma_append_count s1 s2
 val lemma_slice_cons: #a:Type -> s:seq a -> i:nat -> j:nat{i < j && j <= length s}
   -> Lemma (ensures (forall x. mem x (slice s i j) <==> (x = index s i || mem x (slice s (i + 1) j))))
 let lemma_slice_cons #a s i j =
-  cut (Eq (slice s i j) (append (create 1 (index s i)) (slice s (i + 1) j)));
+  cut (equal (slice s i j) (append (create 1 (index s i)) (slice s (i + 1) j)));
   lemma_mem_append (create 1 (index s i)) (slice s (i + 1) j)
 
 val lemma_slice_snoc: #a:Type -> s:seq a -> i:nat -> j:nat{i < j && j <= length s}
   -> Lemma (ensures (forall x. mem x (slice s i j) <==> (x = index s (j - 1) || mem x (slice s i (j - 1)))))
 let lemma_slice_snoc #a s i j =
-  cut (Eq (slice s i j) (append (slice s i (j - 1)) (create 1 (index s (j - 1)))));
+  cut (equal (slice s i j) (append (slice s i (j - 1)) (create 1 (index s (j - 1)))));
   lemma_mem_append (slice s i (j - 1)) (create 1 (index s (j - 1)))
 
 val lemma_ordering_lo_snoc: #a:Type -> f:tot_ord a -> s:seq a -> i:nat -> j:nat{i <= j && j < length s} -> pv:a
    -> Lemma (requires ((forall y. mem y (slice s i j) ==> f y pv) /\ f (index s j) pv))
             (ensures ((forall y. mem y (slice s i (j + 1)) ==> f y pv)))
 let lemma_ordering_lo_snoc #a f s i j pv =
-  cut (Eq (slice s i (j + 1)) (append (slice s i j) (create 1 (index s j))));
+  cut (equal (slice s i (j + 1)) (append (slice s i j) (create 1 (index s j))));
   lemma_mem_append (slice s i j) (create 1 (index s j))
 
 val lemma_ordering_hi_cons: #a:Type -> f:tot_ord a -> s:seq a -> back:nat -> len:nat{back < len && len <= length s} -> pv:a
    -> Lemma (requires ((forall y. mem y (slice s (back + 1) len) ==> f pv y) /\ f pv (index s back)))
             (ensures ((forall y. mem y (slice s back len) ==> f pv y)))
 let lemma_ordering_hi_cons #a f s back len pv =
-  cut (Eq (slice s back len) (append (create 1 (index s back)) (slice s (back + 1) len)));
+  cut (equal (slice s back len) (append (create 1 (index s back)) (slice s (back + 1) len)));
   lemma_mem_append (create 1 (index s back)) (slice s (back + 1) len)
 
 #set-options "--max_fuel 0 --initial_fuel 0"
 val swap_frame_lo : #a:Type -> s:seq a -> lo:nat -> i:nat{lo <= i} -> j:nat{i <= j && j < length s}
      -> Lemma (ensures (slice s lo i == slice (swap s i j) lo i))
-let swap_frame_lo #a s lo i j = cut (Eq (slice s lo i) (slice (swap s i j) lo i))
+let swap_frame_lo #a s lo i j = cut (equal (slice s lo i) (slice (swap s i j) lo i))
 
 val swap_frame_lo' : #a:Type -> s:seq a -> lo:nat -> i':nat {lo <= i'} -> i:nat{i' <= i} -> j:nat{i <= j && j < length s}
      -> Lemma (ensures (slice s lo i' == slice (swap s i j) lo i'))
-let swap_frame_lo' #a s lo i' i j = cut (Eq (slice s lo i') (slice (swap s i j) lo i'))
+let swap_frame_lo' #a s lo i' i j = cut (equal (slice s lo i') (slice (swap s i j) lo i'))
 
 val swap_frame_hi : #a:Type -> s:seq a -> i:nat -> j:nat{i <= j} -> k:nat{j < k} -> hi:nat{k <= hi /\ hi <= length s}
      -> Lemma (ensures (slice s k hi == slice (swap s i j) k hi))
-let swap_frame_hi #a s i j k hi = cut (Eq (slice s k hi) (slice (swap s i j) k hi))
+let swap_frame_hi #a s i j k hi = cut (equal (slice s k hi) (slice (swap s i j) k hi))
 
 val lemma_swap_slice_commute  : #a:Type -> s:seq a -> start:nat -> i:nat{start <= i} -> j:nat{i <= j} -> len:nat{j < len && len <= length s}
     -> Lemma (ensures (slice (swap s i j) start len == (swap (slice s start len) (i - start) (j - start))))
 let lemma_swap_slice_commute #a s start i j len = admit()
 (* this often fails with "assertion failed" *)
-(* let lemma_swap_slice_commute s start i j len = cut (Eq (slice (swap s i j) start len) (swap (slice s start len) (i - start) (j - start))) *)
+(* let lemma_swap_slice_commute s start i j len = cut (equal (slice (swap s i j) start len) (swap (slice s start len) (i - start) (j - start))) *)
 
 val lemma_swap_permutes_slice : #a:Type -> s:seq a -> start:nat -> i:nat{start <= i} -> j:nat{i <= j} -> len:nat{j < len && len <= length s}
    -> Lemma (ensures (permutation a (slice s start len) (slice (swap s i j) start len)))
@@ -322,59 +322,59 @@ let splice #a s1 i s2 j = Seq.append (slice s1 0 i) (Seq.append (slice s2 i j) (
 val splice_refl : #a:Type -> s:seq a -> i:nat -> j:nat{i <= j && j <= length s}
   -> Lemma
   (ensures (s == splice s i s j))
-let splice_refl #a s i j = cut (Eq s (splice s i s j))
+let splice_refl #a s i j = cut (equal s (splice s i s j))
 
 val lemma_swap_splice : #a:Type -> s:seq a -> start:nat -> i:nat{start <= i} -> j:nat{i <= j} -> len:nat{j < len && len <= length s}
    -> Lemma
         (ensures (swap s i j == splice s start (swap s i j) len))
-let lemma_swap_splice #a s start i j len = cut (Eq (swap s i j) (splice s start (swap s i j) len))
+let lemma_swap_splice #a s start i j len = cut (equal (swap s i j) (splice s start (swap s i j) len))
 
 val lemma_seq_frame_hi: #a:Type -> s1:seq a -> s2:seq a{length s1 = length s2} -> i:nat -> j:nat{i <= j} -> m:nat{j <= m} -> n:nat{m < n && n <= length s1}
   -> Lemma
   (requires (s1 == (splice s2 i s1 j)))
   (ensures  ((slice s1 m n == slice s2 m n) /\ (index s1 m == index s2 m)))
 let lemma_seq_frame_hi #a s1 s2 i j m n =
-  cut (Eq (slice s1 m n) (slice s2 m n))
+  cut (equal (slice s1 m n) (slice s2 m n))
 
 val lemma_seq_frame_lo: #a:Type -> s1:seq a -> s2:seq a{length s1 = length s2} -> i:nat -> j:nat{i <= j} -> m:nat{j < m} -> n:nat{m <= n && n <= length s1}
   -> Lemma
   (requires (s1 == (splice s2 m s1 n)))
   (ensures  ((slice s1 i j == slice s2 i j) /\ (index s1 j == index s2 j)))
 let lemma_seq_frame_lo #a s1 s2 i j m n =
-  cut (Eq (slice s1 i j) (slice s2 i j))
+  cut (equal (slice s1 i j) (slice s2 i j))
 
 val lemma_tail_slice: #a:Type -> s:seq a -> i:nat -> j:nat{i < j && j <= length s}
   -> Lemma
   (ensures (tail (slice s i j) == slice s (i + 1) j))
 let lemma_tail_slice #a s i j =
-  cut (Eq (tail (slice s i j)) (slice s (i + 1) j))
+  cut (equal (tail (slice s i j)) (slice s (i + 1) j))
 
 val lemma_weaken_frame_right : #a:Type -> s1:seq a -> s2:seq a{length s1 = length s2} -> i:nat -> j:nat -> k:nat{i <= j && j <= k && k <= length s1}
   -> Lemma
   (requires (s1 == splice s2 i s1 j))
   (ensures (s1 == splice s2 i s1 k))
-let lemma_weaken_frame_right #a s1 s2 i j k = cut (Eq s1 (splice s2 i s1 k))
+let lemma_weaken_frame_right #a s1 s2 i j k = cut (equal s1 (splice s2 i s1 k))
 
 val lemma_weaken_frame_left : #a:Type -> s1:seq a -> s2:seq a{length s1 = length s2} -> i:nat -> j:nat -> k:nat{i <= j && j <= k && k <= length s1}
   -> Lemma
   (requires (s1 == splice s2 j s1 k))
   (ensures (s1 == splice s2 i s1 k))
-let lemma_weaken_frame_left #a s1 s2 i j k = cut (Eq s1 (splice s2 i s1 k))
+let lemma_weaken_frame_left #a s1 s2 i j k = cut (equal s1 (splice s2 i s1 k))
 
 val lemma_trans_frame : #a:Type -> s1:seq a -> s2:seq a -> s3:seq a{length s1 = length s2 /\ length s2 = length s3} -> i:nat -> j:nat{i <= j && j <= length s1}
   -> Lemma
   (requires ((s1 == splice s2 i s1 j) /\ s2 == splice s3 i s2 j))
   (ensures (s1 == splice s3 i s1 j))
-let lemma_trans_frame #a s1 s2 s3 i j = cut (Eq s1 (splice s3 i s1 j))
+let lemma_trans_frame #a s1 s2 s3 i j = cut (equal s1 (splice s3 i s1 j))
 
 val lemma_weaken_perm_left: #a:Type -> s1:seq a -> s2:seq a{length s1 = length s2} -> i:nat -> j:nat -> k:nat{i <= j /\ j <= k /\ k <= length s1}
   -> Lemma
   (requires (s1 == splice s2 j s1 k /\ permutation a (slice s2 j k) (slice s1 j k)))
   (ensures (permutation a (slice s2 i k) (slice s1 i k)))
 let lemma_weaken_perm_left #a s1 s2 i j k =
-  cut (Eq (slice s2 i k) (append (slice s2 i j)
+  cut (equal (slice s2 i k) (append (slice s2 i j)
                                  (slice s2 j k)));
-  cut (Eq (slice s1 i k) (append (slice s2 i j)
+  cut (equal (slice s1 i k) (append (slice s2 i j)
                                  (slice s1 j k)));
   lemma_append_count (slice s2 i j) (slice s2 j k);
   lemma_append_count (slice s2 i j) (slice s1 j k)
@@ -384,9 +384,9 @@ val lemma_weaken_perm_right: #a:Type -> s1:seq a -> s2:seq a{length s1 = length 
   (requires (s1 == splice s2 i s1 j /\ permutation a (slice s2 i j) (slice s1 i j)))
   (ensures (permutation a (slice s2 i k) (slice s1 i k)))
 let lemma_weaken_perm_right #a s1 s2 i j k =
-  cut (Eq (slice s2 i k) (append (slice s2 i j)
+  cut (equal (slice s2 i k) (append (slice s2 i j)
                                  (slice s2 j k)));
-  cut (Eq (slice s1 i k) (append (slice s1 i j)
+  cut (equal (slice s1 i k) (append (slice s1 i j)
                                  (slice s2 j k)));
   lemma_append_count (slice s2 i j) (slice s2 j k);
   lemma_append_count (slice s1 i j) (slice s2 j k)
